theories/lang.v
@@ -10,7 +10,9 @@ From iris.proofmode Require Import tactics.
 
 (* Helper tactics *)
 Ltac inv H := inversion H; subst; clear H.
-Ltac rw_inj H0 H1 := rewrite H0 in H1; injection H1; intros; subst; clear H1.
+
+(* GLOBAL TODO: remove some rewrite map_Forall_lookup that might not be
+ * necessary *)
 
 Definition tag := string.
 
@@ -115,45 +117,111 @@ Fixpoint subst_ty (targs:list lang_ty) (ty: lang_ty):  lang_ty :=
   | ClassT cname cargs => ClassT cname (subst_ty targs <$> cargs)
   | UnionT s t => UnionT (subst_ty targs s) (subst_ty targs t)
   | InterT s t => InterT (subst_ty targs s) (subst_ty targs t)
-  | GenT n => default NothingT (targs !! n)
+  | GenT n => default ty (targs !! n)
   | ExT _ | IntT | BoolT | NothingT | MixedT | NullT | NonNullT => ty
   end.
 
+Lemma subst_ty_nil ty : subst_ty [] ty = ty.
+Proof.
+  induction ty as [ | | | | cname targs hi | | | s t hs ht |
+      s t hs ht | n | cname ] => //=.
+  - rewrite Forall_forall in hi.
+    f_equal.
+    induction targs as [ | hd tl hi2] => //=.
+    f_equal.
+    + apply hi; by constructor.
+    + apply hi2 => h hin.
+      apply hi; by constructor.
+  - by rewrite hs ht.
+  - by rewrite hs ht.
+Qed.
+
+Lemma fmap_subst_ty_nil (σ: stringmap lang_ty): subst_ty [] <$> σ = σ.
+Proof.
+  induction σ as [| s ty ftys Hs IH] using map_ind; first by rewrite fmap_empty.
+  by rewrite fmap_insert subst_ty_nil IH.
+Qed.
+
 Lemma subst_ty_subst ty l k:
+  bounded (length k) ty →
   subst_ty l (subst_ty k ty) = subst_ty (subst_ty l <$> k) ty.
 Proof.
+  move => hbounded.
   induction ty as [ | | | | cname targs hi | | | s t hs ht |
       s t hs ht | n | cname ] => //=.
   - f_equal.
     rewrite -list_fmap_compose.
     rewrite Forall_forall in hi.
     apply map_ext_in => s /elem_of_list_In hin.
-    by apply hi.
-  - by f_equal.
-  - by f_equal.
-  - destruct (k !! n) as [ ty | ] eqn:hty.
-    + by rewrite /= list_lookup_fmap hty.
-    + by rewrite /= list_lookup_fmap hty.
+    apply hi => //.
+    inv hbounded.
+    rewrite Forall_forall in H0.
+    by apply H0.
+  - inv hbounded.
+    f_equal; by eauto.
+  - inv hbounded.
+    f_equal; by eauto.
+  - rewrite list_lookup_fmap.
+    destruct (k !! n) as [ ty | ] eqn:hty => //=.
+    inv hbounded.
+    apply lookup_lt_is_Some_2 in H0.
+    rewrite hty in H0.
+    by elim H0.
 Qed.
 
 Lemma map_subst_ty_subst (j k l: list lang_ty):
+  Forall (bounded (length k)) l →
   subst_ty j <$> (subst_ty k <$> l) =
   subst_ty (subst_ty j <$> k) <$> l.
 Proof.
+  move => hwf.
   induction l as [ | hd tl hi] => //=.
-  rewrite subst_ty_subst.
+  inv hwf.
+  rewrite subst_ty_subst => //.
   f_equal.
   by rewrite list_fmap_compose -/subst_ty list_fmap_id -/fmap hi.
 Qed.
 
 Lemma fmap_subst_ty_subst j k (l: stringmap lang_ty):
+  map_Forall (λ _, bounded (length k)) l →
   subst_ty j <$> (subst_ty k <$> l) =
   subst_ty (subst_ty j <$> k) <$> l.
 Proof.
-  move: j k.
-  induction l as [| s ty ftys Hs IH] using map_ind => j k;
+  move => hwf.
+  move: j k hwf.
+  induction l as [| s ty ftys Hs IH] using map_ind => j k hwf;
     first by rewrite !fmap_empty.
-  by rewrite !fmap_insert subst_ty_subst IH.
+  rewrite map_Forall_insert // in hwf.
+  destruct hwf as [hhd htl].
+  by rewrite !fmap_insert subst_ty_subst // IH.
+Qed.
+
+Lemma bounded_subst n ty:
+  bounded n ty →
+  ∀ m targs, length targs = n →
+  Forall (bounded m) targs →
+  bounded m (subst_ty targs ty).
+Proof.
+  induction ty as [ | | | | cname targs hi | | | s t hs ht |
+      s t hs ht | k | cname ] => //= hb m σ hlen hσ.
+  - constructor.
+    rewrite Forall_forall => ty /elem_of_list_fmap hin.
+    destruct hin as [ty' [-> hin]].
+    rewrite Forall_forall in hi.
+    apply hi with (m := m) (targs := σ) in hin => //.
+    inv hb.
+    rewrite Forall_forall in H0.
+    by apply H0.
+  - inv hb.
+    constructor; by eauto.
+  - inv hb.
+    constructor; by eauto.
+  - inv hb.
+    rewrite Forall_forall in hσ.
+    apply hσ.
+    apply lookup_lt_is_Some_2 in H0.
+    destruct (σ !! k) as [ ty | ] eqn:hty; last by elim H0.
+    by apply elem_of_list_lookup_2 in hty.
 Qed.
 
 Definition var := string.
@@ -180,7 +248,7 @@ Inductive cmd : Set :=
   | NewC (lhs: var) (class_name: tag) (args: stringmap expr)
   | GetC (lhs: var) (recv: expr) (name: string)
   | SetC (recv: expr) (fld: string) (rhs: expr)
-      (* tag test "if ($v is C) { ... }" *)
+      (* tag test "if ($v is C<_>) { ... }" *)
   | CondTagC (v : var) (t : tag) (body : cmd)
 .
 
@@ -200,14 +268,46 @@ Definition subst_mdef targs mdef : methodDef := {|
     methodret := mdef.(methodret);
   |}.
 
+Lemma subst_mdef_body mdef σ: methodbody (subst_mdef σ mdef) = methodbody mdef.
+Proof. by []. Qed.
+
+Lemma subst_mdef_ret mdef σ: methodret (subst_mdef σ mdef) = methodret mdef.
+Proof. by []. Qed.
+
+Lemma subst_mdef_nil mdef : subst_mdef [] mdef = mdef.
+Proof.
+ rewrite /subst_mdef fmap_subst_ty_nil subst_ty_nil.
+ by case mdef.
+Qed.
+
+(* Wf defintions on the source *)
+Definition mdef_bounded n mdef : Prop :=
+  map_Forall (λ _argname, bounded n) mdef.(methodargs) ∧ bounded n mdef.(methodrettype).
+
 Lemma subst_mdef_mdef k l mdef :
+  mdef_bounded (length l) mdef →
   subst_mdef k (subst_mdef l mdef) = subst_mdef (subst_ty k <$> l) mdef.
 Proof.
+  rewrite /mdef_bounded map_Forall_lookup.
+  case => hargs hret.
   rewrite /subst_mdef; destruct mdef as [? args ret ? ?]; f_equiv => //=.
   - by rewrite fmap_subst_ty_subst.
   - by rewrite subst_ty_subst.
 Qed.
 
+Lemma bounded_subst_mdef n mdef:
+  mdef_bounded n mdef →
+  ∀ m targs, length targs = n →
+  Forall (bounded m) targs →
+  mdef_bounded m (subst_mdef targs mdef).
+Proof.
+  move => [/map_Forall_lookup hargs hret] m σ hl hf.
+  rewrite /mdef_bounded /subst_mdef /=; split; last by apply bounded_subst with n.
+  rewrite map_Forall_lookup => k ty hty.
+  apply lookup_fmap_Some in hty as [ty' [ <- hm]].
+  apply bounded_subst with n => //.
+  by eapply hargs.
+Qed.
 
 Record classDef := {
   classname: tag;
@@ -217,74 +317,30 @@ Record classDef := {
   classmethods : stringmap methodDef;
 }.
 
-(* Wf defintions on the source *)
-Definition mdef_bounded n mdef : Prop :=
-  map_Forall (λ _argname, bounded n) mdef.(methodargs) ∧ bounded n mdef.(methodrettype).
-
-Definition cdef_methods_bounded cdef : Prop :=
-  map_Forall (λ _mname mdef, mdef_bounded cdef.(generics) mdef) cdef.(classmethods).
-
 (* "Identity" substitution for n generics *)
-Fixpoint gen_targs_ nleft n : list lang_ty :=
-  match nleft with
-  | O => []
-  | S nleft => GenT n :: gen_targs_ nleft (S n)
-  end.
+Definition gen_targs n : list lang_ty := map GenT (seq 0 n).
 
-Lemma length_gen_targs_: ∀ nleft n, length (gen_targs_ nleft n) = nleft.
-Proof.
-  elim => [ | nleft hi] n //=.
-  by rewrite hi.
-Qed.
-
-Lemma lookup_gen_targs__lt :
-  ∀ nleft n pos, pos < nleft →
-  gen_targs_ nleft n !! pos = Some (GenT (n + pos)).
-Proof.
-  elim => [ | nleft hi] n pos //=; first by lia.
-  case: pos hi => [ | pos] hi //=.
-  { move => _; by rewrite plus_comm. }
-  move/lt_S_n => hlt.
-  apply (hi (S n)) in hlt.
-  rewrite hlt.
-  do 2 f_equal.
-  by lia.
-Qed.
-
-Lemma lookup_gen_targs__ge:
-  ∀ nleft n pos, pos >= nleft →
-  gen_targs_ nleft n !! pos = None.
-Proof.
-  elim => [ | nleft hi] n pos //= hge.
-  case: pos hge => [ | pos] hge; first by lia.
-  simpl.
-  rewrite (hi (S n)) //.
-  by lia.
-Qed.
-
-Definition gen_targs n : list lang_ty := gen_targs_ n 0.
-
-Corollary lookup_gen_targs_lt :
+Lemma lookup_gen_targs_lt :
   ∀ n pos, pos < n → gen_targs n !! pos = Some (GenT pos).
 Proof.
-  rewrite /gen_targs => n pos h.
-  by rewrite lookup_gen_targs__lt.
+  move => n pos h.
+  by rewrite /gen_targs list_lookup_fmap lookup_seq_lt.
 Qed.
 
-Corollary lookup_gen_targs_ge :
+Lemma lookup_gen_targs_ge :
   ∀ n pos, pos ≥ n → gen_targs n !! pos = None.
 Proof.
-  rewrite /gen_targs => n pos h.
-  by rewrite lookup_gen_targs__ge.
+  move => n pos h.
+  by rewrite /gen_targs list_lookup_fmap lookup_seq_ge.
 Qed.
 
-Corollary length_gen_targs n : length (gen_targs n) = n.
-Proof. by rewrite /gen_targs length_gen_targs_. Qed.
+Lemma length_gen_targs n : length (gen_targs n) = n.
+Proof. by rewrite /gen_targs map_length seq_length. Qed.
 
 Corollary gen_targs_O : gen_targs 0 = [].
 Proof. done. Qed.
 
-Lemma subst_gen_targs_is_bounded n ty:
+Lemma subst_ty_id n ty:
   bounded n ty →
   subst_ty (gen_targs n) ty = ty.
 Proof.
@@ -304,6 +360,37 @@ Proof.
   - inv h; f_equal; by eauto.
   - inv h.
     by rewrite lookup_gen_targs_lt.
+Qed.
+
+Lemma subst_tys_id n σ:
+  Forall (bounded n) σ →
+  subst_ty (gen_targs n) <$> σ = σ.
+Proof.
+  revert n.
+  induction σ as [ | hd tl hi] => σ //= hf.
+  f_equal.
+  - apply subst_ty_id.
+    apply Forall_inv in hf.
+    by apply hf.
+  - apply hi.
+    by apply Forall_inv_tail in hf.
+Qed.
+
+Lemma fmap_subst_tys_id n (m: stringmap lang_ty):
+  map_Forall (λ _, bounded n) m →
+  subst_ty (gen_targs n) <$> m = m.
+Proof.
+  revert n.
+  induction m as [| s ty ftys Hs IH] using map_ind => n hm; first by rewrite fmap_empty.
+  rewrite fmap_insert; f_equal.
+  - apply subst_ty_id.
+    apply hm with s.
+    by rewrite lookup_insert.
+  - apply IH.
+    rewrite map_Forall_lookup => k tk hk.
+    apply hm with k.
+    rewrite lookup_insert_ne // => heq; subst.
+    by rewrite Hs in hk.
 Qed.
 
 Lemma subst_ty_gen_targs n targs :
@@ -328,14 +415,24 @@ Lemma subst_mdef_gen_targs_is_bounded n mdef :
   subst_mdef (gen_targs n) mdef = mdef.
 Proof.
   rewrite /mdef_bounded /subst_mdef; move => [/map_Forall_lookup hargs hret].
-  rewrite subst_gen_targs_is_bounded => //.
+  rewrite subst_ty_id => //.
   replace (subst_ty (gen_targs n) <$> methodargs mdef) with (methodargs mdef);
     first by destruct mdef.
   apply map_eq => k.
   rewrite lookup_fmap.
   destruct (methodargs mdef !! k) as [ty | ] eqn:hty => //=.
   apply hargs in hty.
-  by rewrite subst_gen_targs_is_bounded.
+  by rewrite subst_ty_id.
+Qed.
+
+Lemma bounded_gen_targs n: Forall (bounded n) (gen_targs n).
+Proof.
+  rewrite Forall_forall => ty.
+  rewrite /gen_targs => h.
+  apply elem_of_list_fmap_2 in h as [ k [-> hk]].
+  constructor.
+  rewrite elem_of_seq /= in hk.
+  by destruct hk.
 Qed.
 
 (* A program is a collection of classes *)
@@ -346,6 +443,92 @@ Section ProgDef.
   (* assume a given set of class definitions *)
   Context `{PDC: ProgDefContext}.
 
+  Inductive wf_ty : lang_ty → Prop :=
+    | WfInt : wf_ty IntT
+    | WfBool : wf_ty BoolT
+    | WfNothing : wf_ty NothingT
+    | WfMixed : wf_ty MixedT
+    | WfClassT t σ def:
+        Δ !! t = Some def →
+        length σ = def.(generics) →
+        (∀ k ty, σ !! k = Some ty → wf_ty ty) →
+        wf_ty (ClassT t σ)
+    | WfNull : wf_ty NullT
+    | WfNonNull : wf_ty NonNullT
+    | WfUnion s t : wf_ty s → wf_ty t → wf_ty (UnionT s t)
+    | WfInter s t : wf_ty s → wf_ty t → wf_ty (InterT s t)
+    | WfGen k: wf_ty (GenT k)
+    | WfEx t : wf_ty (ExT t)
+  .
+
+  Hint Constructors wf_ty : core.
+
+  Lemma wf_ty_class_inv t σ:
+    wf_ty (ClassT t σ) →
+    Forall wf_ty σ.
+  Proof.
+    move => h.
+    inv h.
+    apply Forall_forall => ty hin.
+    apply elem_of_list_lookup_1 in hin.
+    destruct hin as [k hk].
+    by apply H3 in hk.
+  Qed.
+
+  Lemma wf_ty_subst σ ty :
+    Forall wf_ty σ →
+    wf_ty ty → wf_ty (subst_ty σ ty).
+  Proof.
+    move => hwf.
+    induction 1 as [ | | | | t targs def hdef hl h hi | | |
+        s t hs his ht hit | s t hs his ht hit | | ] => //=; try (by constructor).
+    - econstructor; [ done | by rewrite map_length | ].
+      move => k ty.
+      rewrite list_lookup_fmap.
+      destruct (targs !! k) as [ tk | ] eqn:htk => //=.
+      case => <-.
+      by eapply hi.
+    - destruct (σ !! k) as [ ty | ] eqn:hty => /=; last by constructor.
+      rewrite Forall_forall in hwf; apply hwf.
+      by apply elem_of_list_lookup_2 in hty.
+  Qed.
+
+  Lemma wf_ty_subst_map σ σ':
+    Forall wf_ty σ →
+    Forall wf_ty σ' →
+    Forall wf_ty (subst_ty σ <$> σ').
+  Proof.
+    move => h h'.
+    induction σ' as [ | hd tl hi ] => //=.
+    constructor.
+    - apply Forall_inv in h'.
+      by apply wf_ty_subst.
+    - apply hi.
+      by apply Forall_inv_tail in h'.
+  Qed.
+
+  Lemma gen_targs_wf n k ty: gen_targs n !! k = Some ty → wf_ty ty.
+  Proof.
+    rewrite /gen_targs -/fmap => hx.
+    apply list_lookup_fmap_inv in hx.
+    destruct hx as [ty' [ -> h]].
+    by constructor.
+  Qed.
+
+  Definition wf_cdef_parent (prog: stringmap classDef) cdef : Prop :=
+    match cdef.(superclass) with
+    | None => True
+    | Some (parent, σ) =>
+        ∃ pdef, prog !! parent = Some pdef ∧
+        length σ = pdef.(generics) ∧
+        Forall wf_ty σ ∧
+        Forall (bounded cdef.(generics)) σ
+    end
+  .
+  
+  Definition cdef_methods_bounded cdef : Prop :=
+    map_Forall (λ _mname mdef, mdef_bounded cdef.(generics) mdef) cdef.(classmethods).
+
   (* source relation `class A<...> extends B<...>` *)
   Inductive extends_using : tag → tag → list lang_ty → Prop :=
     | ExtendsUsing A B cdef σB:
@@ -355,6 +538,25 @@ Section ProgDef.
 
   Hint Constructors extends_using : core.
 
+  Lemma extends_using_wf A B σ:
+    map_Forall (λ _cname, wf_cdef_parent Δ) Δ →
+    extends_using A B σ →
+    ∃ adef bdef,
+    Δ !! A = Some adef ∧
+    Δ !! B = Some bdef ∧
+    Forall (bounded adef.(generics)) σ ∧
+    length σ = bdef.(generics) ∧
+    Forall wf_ty σ.
+  Proof.
+    move => /map_Forall_lookup hwf hext.
+    inv hext.
+    assert (H' := H).
+    apply hwf in H.
+    rewrite /wf_cdef_parent H0 in H.
+    destruct H as (pdef & h & hlen & hσ & hf).
+    by exists cdef, pdef.
+  Qed.
+    
   Inductive extends: tag → tag → Prop :=
     | Extends A B cdef σB:
         Δ !! A = Some cdef →
@@ -363,42 +565,269 @@ Section ProgDef.
 
   Hint Constructors extends : core.
 
+  Definition inherits := rtc extends.
+
   Inductive inherits_using : tag → tag → list lang_ty → Prop :=
+    | InheritsRefl A adef:
+        Δ !! A = Some adef →
+        inherits_using A A (gen_targs (adef.(generics)))
     | InheritsExtends A B σ:
         extends_using A B σ →
         inherits_using A B σ
     | InheritsTrans A B σB C σC:
-        inherits_using A B σB →
+        extends_using A B σB →
         inherits_using B C σC →
         inherits_using A C (subst_ty σB <$> σC)
   .
 
   Hint Constructors inherits_using : core.
 
-  Definition inherits := rtc extends.
+  Lemma inherits_using_wf A B σ:
+    map_Forall (λ _cname, wf_cdef_parent Δ) Δ →
+    inherits_using A B σ →
+    ∃ adef bdef,
+    Δ !! A = Some adef ∧
+    Δ !! B = Some bdef ∧
+    Forall (bounded adef.(generics)) σ ∧
+    length σ = bdef.(generics) ∧
+    Forall wf_ty σ.
+  Proof.
+    move => hwf.
+    induction 1 as [ A adef hΔ | A B σ hext | A B σ C σC hext h hi ].
+    - exists adef, adef; repeat split => //.
+      + by apply bounded_gen_targs.
+      + by rewrite length_gen_targs.
+      + rewrite Forall_forall => x hx.
+        apply elem_of_list_lookup_1 in hx.
+        destruct hx as [i hi].
+        by apply gen_targs_wf in hi.
+    - by apply extends_using_wf.
+    - apply extends_using_wf in hext => //.
+      destruct hext as [adef [bdef [ha0 [hb0 [hf0 [hl0 hσ]]]]]].
+      destruct hi as [? [cdef [hb1 [hc1 [hf1 [hl1 hσC]]]]]].
+      simplify_eq.
+      exists adef, cdef; repeat split => //.
+      + rewrite Forall_forall => ty hin.
+        apply elem_of_list_fmap_2 in hin as [ty' [-> hin]].
+        rewrite Forall_forall in hf1; apply hf1 in hin.
+        by eapply bounded_subst.
+      + by rewrite map_length.
+      + apply Forall_forall => x hx.
+        apply elem_of_list_fmap_2 in hx as [ty [ -> hty]].
+        apply wf_ty_subst => //.
+        rewrite Forall_forall in hσC.
+        by apply hσC in hty.
+  Qed.
+
+  Lemma inherits_using_trans A B C σB σC:
+    map_Forall (λ _cname, wf_cdef_parent Δ) Δ →
+    inherits_using A B σB →
+    inherits_using B C σC →
+    inherits_using A C (subst_ty σB <$> σC).
+  Proof.
+    move => hwf h;
+    move : h C σC.
+    induction 1 as [ A cdef hΔ | A B s hext | A B s C t hext h hi] => Z σ' hin.
+    - rewrite subst_tys_id //.
+      apply inherits_using_wf in hin => //.
+      destruct hin as (? & ? & ? & ? & hF & _ ).
+      by simplify_eq.
+    - by econstructor.
+    - assert (hCZ := hin).
+      apply hi in hin; clear hi.
+      rewrite -map_subst_ty_subst; first by eapply InheritsTrans.
+      apply inherits_using_wf in h => //.
+      apply inherits_using_wf in hCZ => //.
+      destruct h as [bdef [cdef [hB [hC [hF0 [hlen0 _]]]]]].
+      destruct hCZ as [? [zdef [hC' [hZ [hF1 [hlen1 _]]]]]].
+      simplify_eq.
+      by rewrite hlen0.
+  Qed.
+
+  (* Our class inheritance tree/forest doesn't have cycles. Which means
+   * inherits A B → inherits B A → A = B.
+   *)
+  Definition wf_no_cycle (prog: stringmap classDef) :=
+    ∀ A B σ σ', inherits_using A B σ → inherits_using B A σ' → A = B ∧σ = σ'.
+
+  Lemma inherits_using_chain A B σ:
+    map_Forall (λ _cname, wf_cdef_parent Δ) Δ →
+    inherits_using A B σ →
+    ∀ C σ', inherits_using A C σ' →
+    (∃ σ'', (subst_ty σ <$> σ'' = σ' ∧ inherits_using B C σ'') ∨
+            (subst_ty σ' <$> σ'' = σ ∧ inherits_using C B σ'')).
+  Proof.
+    move => hwf.
+    induction 1 as [ A adef hΔ | A B s hext | A B s C t hext h hi] => Z σ' hz.
+    - exists σ'; left; split => //.
+      apply subst_tys_id.
+      apply inherits_using_wf in hz => //.
+      destruct hz as (? & ? & ? & ? & hF & _ ).
+      by simplify_eq.
+    - inv hext; inv hz.
+      + simplify_eq.
+        exists s; right; split; last by econstructor; econstructor.
+        apply subst_tys_id.
+        apply hwf in H.
+        rewrite /wf_cdef_parent H0 in H.
+        by destruct H as (? & ? & _ & _ & hF).
+      + inv H1.
+        simplify_eq.
+        apply hwf in H.
+        rewrite /wf_cdef_parent H0 in H.
+        destruct H as (bdef & hB & hL & _ & hF).
+        exists (gen_targs bdef.(generics)); left; split; last by econstructor.
+        by rewrite subst_ty_gen_targs.
+      + inv H1.
+        simplify_eq.
+        exists σC; by left.
+    - destruct (inherits_using_wf _ _ _ hwf hz) as (adef & zdef & hA & hZ & hF0 & hL0 & _).
+      inv hext; inv hz.
+      + simplify_eq.
+        exists (subst_ty s <$> t); right; split; last first.
+        { eapply InheritsTrans => //.
+          by econstructor.
+        }
+        rewrite subst_tys_id // Forall_forall => ty hty.
+        apply elem_of_list_fmap_2 in hty as [ ty' [ -> hty']].
+        apply hwf in hA.
+        rewrite /wf_cdef_parent H0 in hA.
+        destruct hA as (bdef & hB & hL & _ & hF).
+        apply bounded_subst with (generics bdef) => //.
+        apply inherits_using_wf in h => //.
+        destruct h as (? & cdef & ? & hC & hF' & hL' & _); simplify_eq.
+        by rewrite Forall_forall in hF'; apply hF'.
+      + inv H1.
+        simplify_eq.
+        exists t; by right.
+      + inv H1.
+        simplify_eq.
+        apply hi in H2 as [σ'' [ [<- hx] | [<- hx]]]; clear hi.
+        * exists σ''; left; split; last done.
+          rewrite map_subst_ty_subst //.
+          apply inherits_using_wf in h => //.
+          apply inherits_using_wf in hx => //.
+          destruct h as (bdef & Cdef & ? & ? & hf0 & hl0 & _).
+          destruct hx as (? & zdef' & ? & ? & hf1 & hl1 & _).
+          simplify_eq.
+          by rewrite hl0.
+        * exists σ''; right; split; last done.
+          rewrite map_subst_ty_subst //.
+          apply inherits_using_wf in h => //.
+          apply inherits_using_wf in hx => //.
+          destruct h as (bdef & Cdef & ? & ? & hf0 & hl0 & _).
+          destruct hx as (zdef' & ? & ? & ? & hf1 & hl1 & _).
+          simplify_eq.
+          rewrite map_length in hL0.
+          by rewrite hL0.
+  Qed.
+
+  Lemma inherits_using_refl A σ:
+    wf_no_cycle Δ →
+    inherits_using A A σ →
+    ∃ adef, Δ !! A = Some adef ∧ σ = gen_targs adef.(generics).
+  Proof.
+    move => hwf hA.
+    assert (h: ∃ adef, Δ !! A = Some adef).
+    { inv hA.
+      - by exists adef.
+      - inv H.
+        by exists cdef.
+      - inv H.
+        by exists cdef.
+    }
+    destruct h as [adef hΔ].
+    exists adef; split => //.
+    eapply hwf; first by apply hA.
+    by constructor.
+  Qed.
+
+  Lemma inherits_using_fun A B σ:
+    wf_no_cycle Δ →
+    map_Forall (λ _cname, wf_cdef_parent Δ) Δ →
+    inherits_using A B σ →
+    ∀ σ', inherits_using A B σ' → σ = σ'.
+  Proof.
+    move => hwf hp.
+    induction 1 as [ A adef hΔ | A B s hext | A B s C t hext h hi ] => σ' hother.
+    - apply inherits_using_refl in hother as [? [h ->]] => //.
+      by simplify_eq.
+    - inv hext; inv hother.
+      + simplify_eq.
+        destruct (inherits_using_refl B s) as [? [h ->]] => //; last by simplify_eq.
+        eapply InheritsExtends.
+        by econstructor.
+      + inv H1; by simplify_eq.
+      + inv H1; simplify_eq.
+        apply inherits_using_refl in H2 as [bdef [hb ->]] => //.
+        rewrite subst_ty_gen_targs //.
+        apply hp in H.
+        rewrite /wf_cdef_parent H0 in H.
+        destruct H as [? [? [ -> _ ]]].
+        by simplify_eq.
+    - inv hext; inv hother.
+      + simplify_eq.
+        eapply hwf; last by constructor.
+        eapply InheritsTrans; last done.
+        by econstructor.
+      + inv H1; simplify_eq.
+        apply inherits_using_refl in h => //.
+        destruct h as [bdef [hB ->]].
+        rewrite subst_ty_gen_targs //.
+        apply hp in H.
+        rewrite /wf_cdef_parent H0 in H.
+        destruct H as [? [? [ -> _ ]]].
+        by simplify_eq.
+      + inv H1; simplify_eq.
+        apply hi in H2; by subst.
+  Qed.
 
   Lemma inherits_to_using A B:
-    inherits A B → (A = B) ∨ ∃ σ, inherits_using A B σ.
+    map_Forall (λ _cname, wf_cdef_parent Δ) Δ →
+    is_Some (Δ !! A) →
+    inherits A B → ∃ σ, inherits_using A B σ.
   Proof.
-    induction 1 as [ x | x y z hxy hyz hi].
-    - by left.
-    - destruct hi as [-> | [σ hi]]; right.
-      + inv hxy.
-        exists σB; by eauto.
-      + inv hxy.
-        exists (subst_ty σB <$> σ); by eauto.
+    move => /map_Forall_lookup hp h.
+    induction 1 as [ x | s t u hst htu hi ].
+    - destruct h as [ xdef h ].
+      exists (gen_targs xdef.(generics)); by constructor.
+    - inv hst.
+      assert (ht: is_Some (Δ !! t)).
+      {
+        apply hp in H.
+        rewrite /wf_cdef_parent H0 in H.
+        by destruct H as [tdef [-> _]].
+      }
+      apply hi in ht as [σ ht].
+      exists (subst_ty σB <$> σ).
+      eapply InheritsTrans; last done.
+      by econstructor.
+  Qed.
+
+  Lemma inherits_erase A B σ: inherits_using A B σ → inherits A B.
+  Proof.
+    induction 1 as [ A adef | A B σ hext | A B σ C σC hext h hi ] => //.
+    - inv hext.
+      econstructor; last done.
+      by econstructor.
+    - econstructor; last done.
+      inv hext.
+      by econstructor.
   Qed.
 
   Inductive subtype : lang_ty → lang_ty → Prop :=
     | SubMixed : ∀ ty, subtype ty MixedT
-    | SubClass : ∀ A σA B σB, extends_using A B σB →
+    | SubClass : ∀ A σA B σB adef,
+        Δ !! A = Some adef →
+        length σA = adef.(generics) →
+        extends_using A B σB →
         subtype (ClassT A σA) (ClassT B (subst_ty σA <$> σB))
     | SubMixed2: subtype MixedT (UnionT NonNullT NullT)
     | SubIntNonNull: subtype IntT NonNullT
     | SubBoolNonNull: subtype BoolT NonNullT
     | SubClassNonNull: ∀ A targs, subtype (ClassT A targs) NonNullT
-    | SubUnionUpper1 : ∀ s t, subtype s (UnionT s t)
-    | SubUnionUpper2 : ∀ s t, subtype t (UnionT s t)
+    | SubUnionUpper1 : ∀ s t, wf_ty t → subtype s (UnionT s t)
+    | SubUnionUpper2 : ∀ s t, wf_ty s → subtype t (UnionT s t)
         (* TODO: Do we need this one ? *)
     | SubUnionLeast : ∀ s t u, subtype s u → subtype t u → subtype (UnionT s t) u
     | SubInterLower1 : ∀ s t, subtype (InterT s t) s
@@ -406,7 +835,6 @@ Section ProgDef.
     | SubInterGreatest: ∀ s t u, subtype u s → subtype u t → subtype u (InterT s t)
     | SubRefl: ∀ s, subtype s s
     | SubTrans : ∀ s t u, subtype s t → subtype t u → subtype s u
-    | SubExT : ∀ cname targs, subtype (ClassT cname targs) (ExT cname)
   .
   (* TODO: add Nothing <: t ? *)
 
@@ -414,59 +842,114 @@ Section ProgDef.
 
   Notation "s <: t" := (subtype s t) (at level 70, no associativity).
 
-  (* Not used yet *)
-  Inductive is_class : lang_ty → Prop :=
-    | IsClass A σA : is_class (ClassT A σA)
-  .
-
-  Lemma SubClassInherits A B σB:
-    inherits_using A B σB →
-    ∀ σA,
-    (ClassT A σA) <: (ClassT B (subst_ty σA <$> σB)).
+  Lemma subtype_wf A B:
+    map_Forall (λ _cname, wf_cdef_parent Δ) Δ →
+    wf_ty A → A <: B → wf_ty B.
   Proof.
-    induction 1 as [ A B σ hext | A B σB C σC hAB hiAB hBC hiBC ] => σA (*hσA*).
-    - by econstructor.
-    - eapply SubTrans.
-      + by apply hiAB.
-      + rewrite map_subst_ty_subst.
-        by apply hiBC.
+    move => hp hwf.
+    induction 1 as [ ty | A σA B σB adef hΔ hA hext | | | | A args | s t h
+      | s t h | s t u hs his ht hit | s t | s t | s t u hs his ht hit | s
+      | s t u hst hist htu hitu ] => //=; try (by constructor).
+    - inv hext; simplify_eq.
+      rewrite /map_Forall_lookup in hp.
+      apply hp in hΔ.
+      rewrite /wf_cdef_parent H0 in hΔ.
+      destruct hΔ as (bdef & hB & hL & hσB & hb).
+      econstructor; first done.
+      + by rewrite map_length.
+      + move => k ty.
+        rewrite list_lookup_fmap.
+        destruct (σB !! k) as [ tyk | ] eqn:hty => //=.
+        case => <-.
+        apply wf_ty_subst; first by apply wf_ty_class_inv in hwf.
+        rewrite Forall_forall in hσB.
+        apply elem_of_list_lookup_2 in hty.
+        by apply hσB in hty.
+    - inv hwf; by eauto.
+    - inv hwf; by eauto.
+    - inv hwf; by eauto.
+    - constructor; by eauto.
+    - by eauto.
   Qed.
 
   Lemma subtype_subst A B:
-    A <: B → ∀ targs, (subst_ty targs A) <: (subst_ty targs B).
+    map_Forall (λ _cname, wf_cdef_parent Δ) Δ →
+    A <: B → ∀ σ,
+    Forall wf_ty σ →
+    (subst_ty σ A) <: (subst_ty σ B).
   Proof.
-    induction 1 as [ ty | A σA B σB hext | | | | A args | s t | s t
-      | s t u hs his ht hit | s t | s t | s t u hs his ht hit | s
-      | s t u hst hist htu hitu | cname args ] => targs //=.
+    move => hp.
+    induction 1 as [ ty | A σA B σB adef hΔ hA hext | | | | A args | s t h
+      | s t h | s t u hs his ht hit | s t | s t | s t u hs his ht hit | s
+      | s t u hst hist htu hitu ] => σ hσ //=.
     - rewrite map_subst_ty_subst.
-      by constructor.
+      + econstructor => //.
+        by rewrite map_length.
+      + apply extends_using_wf in hext => //.
+      destruct hext as (? & bdef & ? & hB & hF & hL).
+      simplify_eq.
+      by rewrite hA.
+    - constructor.
+      by apply wf_ty_subst.
+    - constructor.
+      by apply wf_ty_subst.
     - constructor; by eauto.
-    - constructor; by eauto.
+    - econstructor; by eauto.
     - econstructor; by eauto.
   Qed.
 
-  Corollary subtype_inst_class A B σA σB σ :
-    (ClassT A σA) <: (ClassT B σB) →
-    (ClassT A (subst_ty σ <$> σA)) <: (ClassT B (subst_ty σ <$> σB)).
-  Proof.
-    move => h.
-    by apply subtype_subst with (targs := σ) in h.
-  Qed.
-
   (* Derived rules *)
-  Lemma subtype_union_comm : ∀ A B, (UnionT A B) <: (UnionT B A).
-  Proof. by auto.  Qed.
+  Lemma subtype_union_comm : ∀ A B,
+    wf_ty A → wf_ty B →
+    (UnionT A B) <: (UnionT B A).
+  Proof. by auto. Qed.
 
-  Lemma subtype_inter_comm : ∀ A B, (InterT A B) <: (InterT B A).
-  Proof. by auto.  Qed.
+  Lemma subtype_inter_comm : ∀ A B,
+    wf_ty A → wf_ty B →
+    (InterT A B) <: (InterT B A).
+  Proof. by auto. Qed.
 
   Lemma subtype_union_assoc:
-    ∀ A B C, (UnionT (UnionT A B) C) <: (UnionT A (UnionT B C)).
-  Proof. by eauto. Qed.
+    ∀ A B C,
+    wf_ty A → wf_ty B → wf_ty C →
+    (UnionT (UnionT A B) C) <: (UnionT A (UnionT B C)).
+  Proof.
+    move => A B C wfA wfB wfC.
+    apply SubUnionLeast; last by eauto.
+    apply SubUnionLeast; last by eauto.
+    apply SubUnionUpper1.
+    constructor; by eauto.
+  Qed.
 
   Lemma subtype_inter_assoc:
-    ∀ A B C, (InterT (InterT A B) C) <: (InterT A (InterT B C)).
-  Proof. by eauto.  Qed.
+    ∀ A B C, 
+    wf_ty A → wf_ty B → wf_ty C →
+    (InterT (InterT A B) C) <: (InterT A (InterT B C)).
+  Proof. by eauto. Qed.
+
+  Lemma subtype_inherits_using A B σ σA adef:
+    map_Forall (λ _ : string, wf_cdef_parent Δ) Δ →
+    Δ !! A = Some adef →
+    length σA = adef.(generics) →
+    inherits_using A B σ →
+    ClassT A σA <: ClassT B (subst_ty σA <$> σ).
+  Proof.
+    move => hp hA hl h.
+    move : h σA adef hA hl.
+    induction 1 as [ A ? h | A B σ0 hext | A B σ0 C σC hext h hi ] => σA ? hA hl.
+    - simplify_eq.
+      by rewrite subst_ty_gen_targs.
+    - by econstructor.
+    - eapply SubTrans; first by eapply SubClass.
+      apply extends_using_wf in hext => //.
+      destruct hext as (? & bdef & hadef' & hbdef & hF0 & hL0 & _).
+      apply inherits_using_wf in h => //.
+      destruct h as (? & cdef & hbdef' & hcdef & hF1 & hL1 & _).
+      simplify_eq.
+      rewrite map_subst_ty_subst; last by rewrite hL0.
+      apply hi with bdef => //.
+      by rewrite map_length.
+  Qed.
 
   Definition local_tys := stringmap lang_ty.
 
@@ -487,6 +970,60 @@ Section ProgDef.
     apply hrz in hA as (C & hC & hsub).
     apply hlr in hC as (B & -> & hsub').
     exists B; by eauto.
+  Qed.
+
+  Lemma lty_sub_insert_1 lhs ty lty0 lty1:
+    lty0 <:< lty1 →
+    <[lhs:=ty]> lty0 <:< <[lhs:=ty]> lty1.
+  Proof.
+    move => h x xty.
+    rewrite lookup_insert_Some.
+    case => [[<- <-] | [hne hin]].
+    - rewrite lookup_insert; by exists ty.
+    - rewrite lookup_insert_ne //.
+      apply h in hin.
+      destruct hin as [B [hin hsub]].
+      by exists B.
+  Qed.
+
+  Lemma lty_sub_insert_2 ty0 ty1 lhs lty:
+    ty0 <: ty1 →
+    <[lhs := ty0]>lty <:< <[lhs := ty1]> lty.
+  Proof.
+    move => hsub k ty.
+    rewrite lookup_insert_Some.
+    case => [[<- <-] | [hne hin]].
+    - exists ty0; by rewrite lookup_insert.
+    - exists ty; by rewrite lookup_insert_ne.
+  Qed.
+
+  Lemma lty_sub_subst σ lty rty:
+    map_Forall (λ _ : string, wf_cdef_parent Δ) Δ →
+    Forall wf_ty σ →
+    lty <:< rty → (subst_ty σ <$> lty) <:< (subst_ty σ <$> rty).
+  Proof.
+    move => hp hσ hsub k A.
+    rewrite lookup_fmap_Some.
+    case => B [<- hk].
+    apply hsub in hk as [ B' [HB' hsub']].
+    exists (subst_ty σ B').
+    rewrite lookup_fmap HB'; split; first done.
+    by apply subtype_subst.
+  Qed.
+
+  (* Not sure it is useful *)
+  Lemma lty_sub_wf lty rty:
+    map_Forall (λ _ : string, wf_cdef_parent Δ) Δ →
+    lty <:< rty →
+    map_Forall (λ _, wf_ty) lty →
+    map_Forall (λ _, wf_ty) rty.
+  Proof.
+    move => hp.
+    rewrite !map_Forall_lookup => hsub h k ty hk.
+    apply hsub in hk.
+    destruct hk as [ty' [ hk hsub']].
+    apply subtype_wf with ty' => //.
+    by apply h in hk.
   Qed.
 
   Inductive has_field (fname: string) : tag -> lang_ty → Prop :=
@@ -511,16 +1048,10 @@ Section ProgDef.
   Proof.
     induction 1 as [ tag cdef typ hΔ hf
       | tag targs parent cdef typ hΔ hf hs h hi ] => typ' h'.
+    - inv h'; by simplify_eq.
     - inv h'.
-      + rw_inj hΔ H.
-        by rw_inj hf H0.
-      + rw_inj hΔ H.
-        rewrite hf in H0; discriminate.
-    - inv h'.
-      + rw_inj hΔ H.
-        rewrite hf in H0; discriminate.
-      + rw_inj hΔ H.
-        rw_inj hs H1.
+      + by simplify_eq.
+      + simplify_eq.
         by rewrite (hi _ H2).
   Qed.
 
@@ -536,6 +1067,26 @@ Section ProgDef.
   Definition wf_cdef_fields_bounded cdef : Prop :=
     map_Forall (λ _fname, bounded cdef.(generics)) cdef.(classfields).
 
+  Definition wf_cdef_fields_wf cdef : Prop :=
+    map_Forall (λ _fname, wf_ty) cdef.(classfields). 
+
+  Lemma has_field_wf f t fty :
+    map_Forall (λ _cname, wf_cdef_parent Δ) Δ →
+    map_Forall (λ _, wf_cdef_fields_wf) Δ →
+    has_field f t fty →
+    wf_ty fty.
+  Proof.
+    move => /map_Forall_lookup hp /map_Forall_lookup hwf.
+    induction 1 as [ tag cdef typ hΔ hf
+      | tag targs parent cdef typ hΔ hf hs h hi ].
+    - apply hwf in hΔ.
+      by apply hΔ in hf.
+    - apply wf_ty_subst => //.
+      apply hp in hΔ.
+      rewrite /wf_cdef_parent hs in hΔ.
+      by destruct hΔ as (pdef & ? & ? & htargs & _).
+  Qed.
+
   Lemma has_field_extends_using f B typ:
     map_Forall (λ _cname, wf_cdef_fields) Δ →
     has_field f B typ →
@@ -550,51 +1101,105 @@ Section ProgDef.
     by eapply hwf.
   Qed.
 
-  (* Naive method lookup: methods are unique. *)
-  Inductive has_method (mname: string) : methodDef → tag → Prop :=
+  Lemma has_field_bounded f t fty:
+    map_Forall (λ _cname, wf_cdef_parent Δ) Δ →
+    map_Forall (λ _cname, wf_cdef_fields_bounded) Δ →
+    has_field f t fty →
+    ∃ def, Δ !! t = Some def ∧ bounded def.(generics) fty.
+  Proof.
+    move => /map_Forall_lookup hwfparent /map_Forall_lookup hwfb.
+    induction 1 as [ tag cdef typ hΔ hf
+      | tag targs parent cdef typ hΔ hf hs h hi ].
+    - exists cdef; split => //.
+      apply hwfb in hΔ.
+      by apply hΔ in hf.
+    - exists cdef; split => //.
+      destruct hi as [pdef [ hp hb]].
+      apply hwfparent in hΔ.
+      rewrite /wf_cdef_parent hs hp in hΔ.
+      destruct hΔ as (? & [= <-] & h0 & _ & h1).
+      by eapply bounded_subst.
+  Qed.
+
+  Lemma has_field_inherits_using f B typ:
+    map_Forall (λ _cname, wf_cdef_parent Δ) Δ →
+    map_Forall (λ _cname, wf_cdef_fields) Δ →
+    map_Forall (λ _cname, wf_cdef_fields_bounded) Δ →
+    has_field f B typ →
+    ∀ A σB,
+    inherits_using A B σB →
+    has_field f A (subst_ty σB typ).
+  Proof.
+    move => hp hfs hfb hf A σB hin.
+    induction hin as [ A adef | A B σ hext | A B σ C σC hext h hi].
+    - rewrite subst_ty_id //.
+      apply has_field_bounded in hf => //.
+      destruct hf as [? [? h]].
+      by simplify_eq.
+    - by eapply has_field_extends_using.
+    - destruct (has_field_bounded _ _ _ hp hfb hf) as (cdef & hcdef & hc).
+      apply hi in hf; clear hi.
+      apply has_field_extends_using with (A := A) (σB := σ) in hf => //.
+      rewrite -subst_ty_subst //.
+      apply inherits_using_wf in h => //.
+      destruct h as (? & ? & ? & ? & ? & h & _).
+      simplify_eq.
+      by rewrite h.
+  Qed.
+
+  (* Method look returning a instantiated method def and the
+   * tag where the method was defined.
+   *)
+  Inductive has_method (mname: string) : tag → tag → methodDef → Prop :=
     | HasMethod tag cdef mdef:
         Δ !! tag = Some cdef →
         cdef.(classmethods) !! mname = Some mdef →
-        has_method mname mdef tag
-    | InheritsMethod tag parent σ cdef mdef:
+        has_method mname tag tag mdef
+    | InheritsMethod tag parent orig σ cdef mdef:
         Δ !! tag = Some cdef →
         cdef.(classmethods) !! mname = None →
         cdef.(superclass) = Some (parent, σ) →
-        has_method mname mdef parent →
-        has_method mname mdef tag
+        has_method mname parent orig mdef →
+        has_method mname tag orig (subst_mdef σ mdef)
   .
 
   Hint Constructors has_method : code.
 
-  (*
-  Lemma has_method_from n m mdef A:
-    mdef_bounded n mdef →
-    has_method m mdef A →
-    ∃ B cdef orig inst,
-    Δ !! B = Some cdef ∧
-    cdef.(classmethods) !! m = Some orig ∧
-    mdef = subst_mdef inst orig ∧
-    inherits A B.
-  Proof.
-    move => hwf.
-    induction 1 as [ tag cdef mdef hΔ hm 
-      | tag parent inst cdef mdef hΔ hm hs h hi].
-    - exists tag, cdef, mdef, (gen_targs n); repeat split => //.
-      by rewrite subst_mdef_gen_targs_is_bounded.
-    - destruct hi as (B & bdef & orig & Binst & hΔ' & horig & heq & hinherits). 
-      exists B, bdef, orig, (subst_ty targs <$> Binst).
-      split; first done.
-      split; first done.
-      split; first by rewrite heq subst_mdef_mdef.
-      econstructor; last first.
-      + change (ClassT B (subst_ty targs <$> Binst)) with
-        (subst_ty targs (ClassT B Binst)).
-        apply inherits_subst.
-        exact hinherits.
-      + by econstructor.
-  Qed.
-   *)
+  Definition mdef_wf mdef : Prop :=
+    map_Forall (λ _mname, wf_ty) mdef.(methodargs) ∧
+    wf_ty mdef.(methodrettype).
 
+  Definition wf_cdef_methods_wf cdef : Prop :=
+    map_Forall (λ _mname, mdef_wf) cdef.(classmethods).
+
+  Lemma has_method_wf m t orig mdef:
+    map_Forall (λ _cname, wf_cdef_parent Δ) Δ →
+    map_Forall (λ _, wf_cdef_methods_wf) Δ →
+    has_method m t orig mdef →
+    map_Forall (λ _mname, wf_ty) mdef.(methodargs) ∧
+    wf_ty mdef.(methodrettype).
+  Proof.
+    move => hp hm.
+    induction 1 as [ tag cdef mdef ht hin |
+        tag parent orig σ cdef mdef ht hin hs h [hia hir] ].
+    - apply hm in ht.
+      by apply ht in hin.
+    - assert (hσ : Forall wf_ty σ).
+      { rewrite map_Forall_lookup in hp.
+        apply hp in ht.
+        rewrite /wf_cdef_parent hs in ht.
+        by destruct ht as (? & ? & ? & ? & ?).
+      }
+      split.
+      + apply map_Forall_lookup => k ty.
+        rewrite lookup_fmap_Some.
+        case => ty' [<- hk].
+        apply wf_ty_subst => //.
+        rewrite map_Forall_lookup in hia.
+        by apply hia in hk.
+      + rewrite /subst_mdef /=.
+        by apply wf_ty_subst.
+  Qed.
 
   (* We allow method override: children can redeclare a method if types
    * are compatible:
@@ -632,104 +1237,246 @@ Section ProgDef.
     - by eapply h1.
   Qed.
 
-  Definition wf_cdef_methods cdef : Prop :=
-    ∀ m mdef superdef super σ,
-    cdef.(superclass) = Some (super, σ) →
-    has_method m superdef super →
-    cdef.(classmethods) !! m = Some mdef →
-    mdef_incl mdef superdef.
+  Lemma mdef_incl_subst mdef0 mdef1 σ :
+    map_Forall (λ _cname, wf_cdef_parent Δ) Δ →
+    Forall wf_ty σ →
+    mdef_incl mdef0 mdef1 →
+    mdef_incl (subst_mdef σ mdef0) (subst_mdef σ mdef1).
+  Proof.
+    move => hp hσ.
+    rewrite /mdef_incl /subst_mdef /=.
+    case => [hdom [hargs hret]]; split; first by rewrite !dom_fmap_L.
+    split; last by apply subtype_subst.
+    move => k A B.
+    rewrite !lookup_fmap_Some.
+    case => tyA [<- hA].
+    case => tyB [<- hB].
+    apply subtype_subst => //.
+    by eapply hargs.
+  Qed.
+
 
   Definition has_fields A (fields: stringmap lang_ty) : Prop :=
     ∀ fname typ, has_field fname A typ ↔ fields !! fname = Some typ.
 
-  (*
-  Lemma has_method_fun: ∀ A name mdef0 mdef1,
-    has_method name mdef0 A → has_method name mdef1 A → mdef0 = mdef1.
+  Lemma has_method_fun: ∀ A name mdef0 mdef1 orig0 orig1,
+    has_method name A orig0 mdef0 → has_method name A orig1 mdef1 →
+    orig0 = orig1 ∧ mdef0 = mdef1.
   Proof.
-    move => A name mdef0 mdef1 h; move: mdef1.
+    move => A name mdef0 mdef1 orig0 orig1 h; move: mdef1.
     induction h as [ current cdef mdef hΔ hm 
-      | current parent inst cdef mdef hΔ hm hs hp hi ] => mdef1 h1.
+      | current parent orig inst cdef mdef hΔ hm hs hp hi ] => mdef1 h1.
+    - inv h1; by simplify_eq.
     - inv h1.
-      + rewrite hΔ in H; injection H; intros; subst; clear hΔ H.
-        rewrite hm in H0; injection H0; intros; by subst.
-      + rewrite hΔ in H; injection H; intros; subst; clear hΔ H.
-        rewrite hm in H0; discriminate H0.
-    - inv h1.
-      + rewrite hΔ in H; injection H; intros; subst; clear hΔ H.
-        rewrite hm in H0; discriminate H0.
-      + rewrite hΔ in H; injection H; intros; subst; clear hΔ H.
-        rewrite hs in H1; injection H1; intros; subst; clear hs H1.
-        apply hi in H2; by subst.
+      + by simplify_eq.
+      + simplify_eq.
+        apply hi in H2 as []; by subst.
   Qed.
-   *)
 
-  Lemma has_field_inherits :
-    map_Forall (fun _ => wf_cdef_fields) Δ →
-    ∀ A B σ, inherits_using A B σ → 
-    ∀ f fty, has_field f B fty → has_field f A (subst_ty σ fty).
+  Definition wf_method_override (prog: stringmap classDef) :=
+    ∀ A B adef bdef m σ mA mB,
+    prog !! A = Some adef →
+    prog !! B = Some bdef →
+    inherits_using A B σ →
+    adef.(classmethods) !! m = Some mA →
+    bdef.(classmethods) !! m = Some mB →
+    mdef_incl mA (subst_mdef σ mB).
+
+  Lemma has_method_from_def A m orig mdef:
+    map_Forall (λ _cname, wf_cdef_parent Δ) Δ →
+    map_Forall (λ _cname, cdef_methods_bounded) Δ →
+    has_method m A orig mdef →
+    ∃ cdef mdef_orig,
+      Δ !! orig = Some cdef ∧
+      cdef.(classmethods) !! m = Some mdef_orig ∧
+      has_method m orig orig mdef_orig ∧
+      ∃ σ, inherits_using A orig σ ∧ mdef = subst_mdef σ mdef_orig.
   Proof.
-    move => wfΔ A B σ h.
-    induction h as [ A B σ hext | A B σB C σC hAB hiAB hBC hiBC]; move => f fty hf.
-    - inv hext.
-      eapply InheritsField => //.
-      apply wfΔ in H.
-      by eapply H.
-    - apply hiBC in hf.
-      apply hiAB in hf.
-      by rewrite -subst_ty_subst.
+    move => /map_Forall_lookup hp /map_Forall_lookup hmb.
+    induction 1 as [ A adef mdef hΔ hm | A parent orig σ cdef mdef hΔ hm hs h hi ].
+    - exists adef, mdef; repeat split => //; first by econstructor.
+      exists (gen_targs adef.(generics)); split; first by constructor.
+      rewrite subst_mdef_gen_targs_is_bounded //.
+      apply hmb in hΔ.
+      by apply hΔ in hm.
+    - destruct hi as (odef & omdef & ho & hom & hdef & [σo [hin ->]]).
+      exists odef, omdef; repeat split => //.
+      exists (subst_ty σ <$> σo); split.
+      { econstructor; last done.
+        by econstructor.
+      }
+      rewrite subst_mdef_mdef //.
+      assert (ho' := ho).
+      apply hmb in ho.
+      apply ho in hom.
+      apply inherits_using_wf in hin as (? & ? & ? & ? & ? & hlen & _) => //.
+      simplify_eq.
+      by rewrite hlen.
   Qed.
 
-  Lemma has_fields_inherits :
-    map_Forall (fun _ => wf_cdef_fields) Δ →
-    ∀ A B σ, inherits_using A B σ → 
-    ∀ Afields Bfields, has_fields A Afields → has_fields B Bfields →
-    ∀ k fty, Bfields !! k = Some fty →
-    Afields !! k = Some (subst_ty σ fty).
+  Lemma has_method_below_orig A m orig mdef:
+    wf_no_cycle Δ →
+    map_Forall (λ _cname, wf_cdef_parent Δ) Δ →
+    map_Forall (λ _cname, cdef_methods_bounded) Δ →
+    has_method m A orig mdef →
+    ∀ B σ σ', inherits_using A B σ → inherits_using B orig σ' →
+    ∃ odef mdefo mdefB,
+    Δ !! orig = Some odef ∧
+    odef.(classmethods) !! m = Some mdefo ∧
+    has_method m B orig mdefB ∧
+    mdefB = subst_mdef σ' mdefo.
   Proof.
-    move => wfΔ A B σ hin Afields Bfields hA hB k fty hk.
-    apply hB in hk.
-    apply has_field_inherits with (A := A) (σ := σ) in hk => //.
-    by apply hA.
+    move => hc hp hb.
+    induction 1 as [ A cdef mdef hΔ hm | A parent orig σ cdef mdef hΔ hm hs h hi ] =>
+          B σA σB hAB hBO.
+    - destruct (hc _ _ _ _ hAB hBO) as [-> ->].
+      apply inherits_using_refl in hAB as [ ? [? ->]] => // ; simplify_eq.
+      exists cdef, mdef, mdef; repeat split => //.
+      + by econstructor.
+      + rewrite subst_mdef_gen_targs_is_bounded //.
+        rewrite map_Forall_lookup in hb.
+        apply hb in hΔ.
+        by apply hΔ in hm.
+    - inv hAB.
+      + simplify_eq.
+        destruct (has_method_from_def _ _ _ _ hp hb h) as (odef & modef & ? & hmo & _ & [σo [hin ->]]).
+        exists odef, modef, (subst_mdef σ (subst_mdef σo modef)); repeat split => //.
+        * by econstructor.
+        * assert (hσ: subst_ty σ <$> σo = σB).
+          { eapply inherits_using_fun => //.
+            eapply InheritsTrans; last done.
+            by econstructor.
+          }
+          rewrite subst_mdef_mdef; first by rewrite hσ.
+          apply inherits_using_wf in hBO as (? & ? & ? & ? & hF & hL & _) => //; simplify_eq.
+          apply hb in H1.
+          apply H1 in hmo.
+          rewrite map_Forall_lookup in hp.
+          rewrite map_length in hL.
+          by rewrite hL.
+      + inv H; simplify_eq; clear hi.
+        destruct (has_method_from_def _ _ _ _ hp hb h) as (odef & modef & ? & hmo & _ & [σo [hin ->]]).
+        exists odef, modef, (subst_mdef σo modef); repeat split => //.
+        replace σB with σo; first done.
+        by eapply inherits_using_fun.
+      + inv H; simplify_eq.
+        destruct (hi _ _ _ H0 hBO) as (odef & mdefo & mdefB & ? & ? & ? & ->).
+        by exists odef, mdefo, (subst_mdef σB mdefo).
   Qed.
 
-  (*
-
-  Corollary has_fields_inherits_lookup:
-    map_Forall (fun _ => wf_cdef_fields) Δ →
-    ∀ A B name fty fields,
-    has_field name fty B →
-    inherits A B →
-    has_fields A fields →
-    fields !! name = Some fty.
+  Lemma has_method_ordered A B σ m origA mdefA origB mdefB:
+    wf_no_cycle Δ →
+    wf_method_override Δ →
+    map_Forall (λ _cname, wf_cdef_parent Δ) Δ →
+    map_Forall (λ _cname, cdef_methods_bounded) Δ →
+    inherits_using A B σ →
+    has_method m A origA mdefA →
+    has_method m B origB mdefB →
+    ∃ σin σA σB oA oB mA mB,
+      subst_ty σ <$> σB = subst_ty σA <$> σin ∧
+      Δ !! origA = Some oA ∧
+      Δ !! origB = Some oB ∧
+      oA.(classmethods) !! m = Some mA ∧
+      oB.(classmethods) !! m = Some mB ∧
+      inherits_using origA origB σin ∧
+      inherits_using A origA σA ∧
+      inherits_using B origB σB ∧
+      has_method m origA origA mA ∧ (* Not sure these are useful *)
+      has_method m origB origB mB ∧
+      mdefA = subst_mdef σA mA ∧
+      mdefB = subst_mdef σB mB ∧
+      mdef_incl mA (subst_mdef σin mB) ∧
+      mdef_incl mdefA (subst_mdef σ mdefB).
   Proof.
-    move => wfΔ A B name fty fields hfields hinherits hf.
-    destruct (hf name fty) as [hl hr].
-    apply hl.
-    by eapply (has_field_inherits wfΔ).
+    move => hc ho hp hm hin hA hB.
+    assert (hhA := hA).
+    assert (hhB := hB).
+    apply has_method_from_def in hA => //.
+    apply has_method_from_def in hB => //.
+    destruct hA as (oadef & oaorig & hoA & hmA & hmoA & [σA [hiA ->]]).
+    destruct hB as (obdef & oborig & hoB & hmB & hmoB & [σB [hiB ->]]).
+    destruct (inherits_using_chain _ _ _ hp hin _ _ hiA) as [σ'' [ [<- h] | [<- h]]].
+    - destruct (has_method_below_orig _ _ _ _ hc hp hm hhA _ _ _ hin h) as
+        (? & ? & mbdef & ? & ? & hbm & ->); simplify_eq.
+      destruct (has_method_fun _ _ _ _ _ _ hhB hbm) as [-> ->].
+      simplify_eq.
+      exists (gen_targs oadef.(generics)),
+             (subst_ty σ <$> σ''),
+             σ'',
+             oadef, oadef,
+             oaorig, oaorig.
+      split.
+      { rewrite subst_ty_gen_targs //.
+        apply inherits_using_wf in hiA => //.
+        repeat destruct hiA as [? hiA]; by simplify_eq.
+      }
+      do 4 (split => //).
+      split; first by econstructor.
+      do 6 (split => //).
+      split.
+      + repeat split.
+        * by rewrite /subst_mdef /= dom_fmap_L.
+        * move => k X Y hX.
+          rewrite /subst_mdef /= lookup_fmap hX /= subst_ty_id.
+          { by case => ->. }
+          apply hm in hoA.
+          apply hoA in hmA.
+          by apply hmA in hX.
+        * rewrite /subst_mdef /= subst_ty_id //.
+          apply hm in hoA.
+          by apply hoA in hmA as [].
+      + rewrite subst_mdef_mdef; first by apply mdef_incl_reflexive.
+        assert (hoA' := hoA).
+        apply hm in hoA'.
+        apply hoA' in hmA.
+        apply inherits_using_wf in h => //.
+        repeat destruct h as [? h]; simplify_eq.
+        by rewrite H2.
+    - exists (subst_ty σ'' <$> σB), σA, σB, oadef, obdef, oaorig, oborig.
+      split.
+      { rewrite map_subst_ty_subst //.
+        apply inherits_using_wf in hiB => //.
+        repeat destruct hiB as [? hiB].
+        apply inherits_using_wf in h => //.
+        repeat destruct h as [? h].
+        simplify_eq.
+        by rewrite H6.
+      }
+      assert (hh: inherits_using origA origB (subst_ty σ'' <$> σB))
+        by (by eapply inherits_using_trans).
+      assert (hincl : mdef_incl oaorig (subst_mdef (subst_ty σ'' <$> σB) oborig))
+        by (by eapply (ho origA origB) in hh).
+      do 12 (split => //).
+      rewrite -subst_mdef_mdef; last first.
+      { assert (hoB' := hoB).
+        apply hm in hoB'.
+        apply hoB' in hmB.
+        apply inherits_using_wf in hiB => //.
+        repeat destruct hiB as [? hiB].
+        simplify_eq.
+        apply bounded_subst_mdef with (generics obdef) => //.
+        apply inherits_using_wf in h => //.
+        repeat destruct h as [? h].
+        simplify_eq.
+        rewrite Forall_forall => ty hty.
+        rewrite H5.
+        rewrite Forall_forall in H1.
+        by apply H1 in hty.
+      }
+      apply mdef_incl_subst => //.
+      { apply inherits_using_wf in hiA => //.
+        by repeat destruct hiA as [? hiA].
+      }
+      rewrite subst_mdef_mdef //.
+      { assert (hoB' := hoB).
+        apply hm in hoB'.
+        apply hoB' in hmB.
+        apply inherits_using_wf in hiB => //.
+        repeat destruct hiB as [? hiB].
+        simplify_eq.
+        by rewrite H2.
+      }
   Qed.
-
-  Lemma has_method_inherits (Hcdef: map_Forall (fun _ => wf_cdef_methods) Δ):
-    ∀ A B, inherits A B →
-    ∀ m mdef, has_method m mdef B →
-    ∃ mdef', has_method m mdef' A ∧ mdef_incl mdef' mdef.
-  Proof.
-    move => A B h.
-    induction h as [ t | x y z hxy hyz hi]; move => m mdef hf.
-    { exists mdef; split => //.
-      by apply mdef_incl_reflexive.
-    }
-    apply hi in hf as (mdef' & hm & hincl).
-    destruct hxy as (cdef & hΔ & hs).
-    destruct (cdef.(classmethods) !! m) as [ mdef'' | ] eqn:heq; last first.
-    { exists mdef'; split; last done.
-      by apply InheritsMethod with y cdef.
-    }
-    exists mdef''; split; first by apply HasMethod with cdef.
-    apply mdef_incl_transitive with mdef'; last done.
-    apply Hcdef in hΔ.
-    by eapply hΔ.
-  Qed.
-   *)
 
   (* Typing Judgements *)
   Definition is_bool_op op : bool :=
@@ -759,9 +1506,38 @@ Section ProgDef.
         expr_has_ty lty (VarE v) ty
     | ESubTy: ∀ e s t,
         expr_has_ty lty e s →
+        wf_ty t →
         s <: t →
         expr_has_ty lty e t
   .
+
+  Lemma expr_has_ty_subst σ lty e ty:
+    map_Forall (λ _ : string, wf_cdef_parent Δ) Δ →
+    Forall wf_ty σ →
+    expr_has_ty lty e ty →
+    expr_has_ty (subst_ty σ <$> lty) e (subst_ty σ ty).
+  Proof.
+    move => hp hwf.
+    induction 1 as [ z | b | | op e1 e2 hop h1 hi1 h2 hi2 |
+      op e1 e2 hop h1 hi1 h2 hi2 | v ty h | e s t h hi hsub ] => //=; try (by constructor).
+    - constructor.
+      by rewrite lookup_fmap h.
+    - econstructor; first by apply hi.
+      + by apply wf_ty_subst.
+      + by apply subtype_subst.
+  Qed.
+
+  Lemma expr_has_ty_wf lty e ty:
+    map_Forall (λ _, wf_ty) lty →
+    expr_has_ty lty e ty →
+    wf_ty ty.
+  Proof.
+    move => hwf.
+    induction 1 as [ z | b | | op e1 e2 hop h1 hi1 h2 hi2 |
+      op e1 e2 hop h1 hi1 h2 hi2 | v ty h | e s t h hi hsub ] => //=; try (by constructor).
+    rewrite map_Forall_lookup in hwf.
+    by apply hwf in h.
+  Qed.
 
   (* continuation-based typing for commands *)
   Inductive cmd_has_ty :
@@ -789,8 +1565,7 @@ Section ProgDef.
         expr_has_ty lty rhs (subst_ty σ fty) →
         cmd_has_ty lty (SetC recv fld rhs) lty
     | NewTy: ∀ lty lhs t targs args fields (*cdef*),
-        (* Δ !! t = Some cdef → *)
-        (* length targs = cdef.(generics) → (1* check constraints *1) *)
+        wf_ty (ClassT t targs) → (* TODO: discuss *)
         has_fields t fields →
         dom (gset string) fields = dom _ args →
         (∀ f fty arg,
@@ -798,69 +1573,197 @@ Section ProgDef.
         args !! f = Some arg →
         expr_has_ty lty arg (subst_ty targs fty)) →
         cmd_has_ty lty (NewC lhs t args) (<[lhs := ClassT t targs]>lty)
-        (*
-    | CallTy: ∀ lty lhs recv t targs name mdef args (*cdef*),
+    | CallTy: ∀ lty lhs recv t targs name orig mdef args (*cdef*),
         (* Δ !! t = Some cdef → *)
         (* length targs = cdef.(generics) → *)
         expr_has_ty lty recv (ClassT t targs) →
-        has_method name mdef t →
+        has_method name t orig mdef →
         dom (gset string) mdef.(methodargs) = dom _ args →
         (∀ x ty arg,
         mdef.(methodargs) !! x = Some ty →
         args !! x = Some arg →
         expr_has_ty lty arg (subst_ty targs ty)) →
         cmd_has_ty lty (CallC lhs recv name args) (<[lhs := subst_ty targs mdef.(methodrettype)]>lty)
-         *)
     | SubTy: ∀ lty c rty rty',
         rty' <:< rty →
         cmd_has_ty lty c rty' →
         cmd_has_ty lty c rty
-    | CondTagTy lty v tv t cmd :
+    | CondTagTy lty rty v tv t cmd :
         lty !! v = Some tv →
-        cmd_has_ty (<[v:=InterT tv (ExT t)]> lty) cmd lty →
-        cmd_has_ty lty (CondTagC v t cmd) lty
+        lty <:< rty →
+        cmd_has_ty (<[v:=InterT tv (ExT t)]> lty) cmd rty →
+        cmd_has_ty lty (CondTagC v t cmd) rty
   .
 
-  (* TODO: update
-  Corollary CallTy_: ∀ lty lhs recv t targs name mdef args,
-    expr_has_ty lty recv (ClassT t targs) →
-    has_method name mdef t →
-    dom (gset string) mdef.(methodargs) = dom _ args →
-    (∀ x ty arg,
-    mdef.(methodargs) !! x = Some ty →
-    args !! x = Some arg →
-    ∃ ty', ty' <: subst_ty targs ty ∧ expr_has_ty lty arg ty') →
-    cmd_has_ty lty (CallC lhs recv name args) (<[lhs := subst_ty targs mdef.(methodrettype)]>lty).
+  Lemma cmd_has_ty_wf lty cmd lty' :
+    map_Forall (λ _ : string, wf_cdef_parent Δ) Δ →
+    map_Forall (λ _ : string, wf_cdef_fields_wf) Δ →
+    map_Forall (λ _ : string, wf_cdef_methods_wf) Δ →
+    map_Forall (λ _, wf_ty) lty →
+    cmd_has_ty lty cmd lty' →
+    map_Forall (λ _, wf_ty) lty'.
   Proof.
-    move => lty lhs recv t targs name mdef args hrecv hmdef hdom hargs.
-    econstructor; [done | done | done | ].
-    move => k ty arg hk ha.
-    destruct (hargs _ _ _ hk ha) as (ty' & hsub & he).
-    by econstructor.
+    move => hp hfields hmethods hwf.
+    induction 1 as [ lty | ????? h1 hi1 h2 hi2 | ???? he |
+      ????? he h1 hi1 h2 hi2 | ??????? he hf |
+      ??????? he hf hr | ?????? ht hf hdom hargs |
+      ????????? he hm hdom hargs |
+      ???? hsub h hi | ?????? hin hr h hi ] => //=; try (by eauto).
+    - apply map_Forall_insert_2 => //.
+      by apply expr_has_ty_wf in he.
+    - apply map_Forall_insert_2 => //.
+      apply wf_ty_subst.
+      + apply expr_has_ty_wf in he => //.
+        by apply wf_ty_class_inv in he.
+      + by apply has_field_wf in hf.
+    - by apply map_Forall_insert_2.
+    - apply map_Forall_insert_2 => //.
+      apply has_method_wf in hm => //.
+      destruct hm as [hargs' hret'].
+      apply wf_ty_subst => //.
+      apply expr_has_ty_wf in he => //.
+      by apply wf_ty_class_inv in he.
+    - apply hi in hwf; clear hi h.
+      rewrite map_Forall_lookup => k ty hty.
+      apply hsub in hty.
+      destruct hty as [ty' [ hty' hsub']].
+      rewrite map_Forall_lookup in hwf; apply hwf in hty'.
+      by eapply subtype_wf.
+    - apply hi; clear hi.
+      rewrite map_Forall_lookup => k ty.
+      rewrite lookup_insert_Some.
+      case => [[heq <-] | [hne hk]].
+      { constructor; last by constructor.
+        by apply hwf in hin.
+      }
+      by apply hwf in hk.
   Qed.
 
-  Lemma CallTyGen: ∀ lty lhs recv t targs name mdef args ret,
-    expr_has_ty lty recv (ClassT t targs) →
-    has_method name mdef t →
-    dom (gset string) mdef.(methodargs) = dom _ args →
-    (∀ x ty arg,
-    mdef.(methodargs) !! x = Some ty →
-    args !! x = Some arg →
-    ∃ ty', ty' <: subst_ty targs ty ∧ expr_has_ty lty arg ty') →
-    subst_ty targs mdef.(methodrettype) <: ret →
-    cmd_has_ty lty (CallC lhs recv name args) (<[lhs := ret]>lty).
+  Lemma cmd_has_ty_subst σ lty cmd lty':
+    map_Forall (λ _ : string, wf_cdef_parent Δ) Δ →
+    map_Forall (λ _ : string, wf_cdef_fields_wf) Δ →
+    map_Forall (λ _ : string, wf_cdef_methods_wf) Δ →
+    map_Forall (λ _ : string, wf_cdef_fields_bounded) Δ →
+    map_Forall (λ _ : string, cdef_methods_bounded) Δ →
+    map_Forall (λ _, wf_ty) lty →
+    Forall wf_ty σ →
+    cmd_has_ty lty cmd lty' →
+    cmd_has_ty (subst_ty σ <$> lty) cmd (subst_ty σ <$> lty').
   Proof.
-    move =>lty lhs ?????? ret hrecv hm hdom hargs hret.
-    eapply SubTy; last by eapply CallTy_.
-    move => k A hA.
-    rewrite lookup_insert_Some in hA.
-    destruct hA as [[<- <-] | [hne heq]].
-    - rewrite lookup_insert.
-      by eexists.
-    - rewrite lookup_insert_ne //.
-      by exists A.
+    move => hp hfields hmethods hfb hmb hwf0 hwf1.
+    induction 1 as [ lty | ????? h1 hi1 h2 hi2 | ???? he |
+      ????? he h1 hi1 h2 hi2 | ??????? he hf |
+      ??????? he hf hr | ?????? hwf hf hdom hargs |
+      ????????? he hm hdom hargs |
+      ???? hsub h hi | ?????? hin hr h hi ] => //=.
+    - by constructor.
+    - econstructor.
+      + by eapply hi1.
+      + eapply hi2.
+        by apply cmd_has_ty_wf in h1.
+    - rewrite fmap_insert.
+      eapply LetTy.
+      by eapply expr_has_ty_subst.
+    - eapply IfTy => //.
+      + change BoolT with (subst_ty σ BoolT).
+        by eapply expr_has_ty_subst.
+      + by apply hi1.
+      + apply hi2.
+        by apply cmd_has_ty_wf in h1.
+    - rewrite fmap_insert subst_ty_subst; last first.
+      { apply has_field_bounded in hf => //.
+        destruct hf as (hdef & ht & hfty).
+        apply expr_has_ty_wf in he => //.
+        inv he; simplify_eq.
+        by rewrite H2.
+      }
+      eapply GetTy; last done.
+      change (ClassT t (subst_ty σ <$> σ0)) with (subst_ty σ (ClassT t σ0)).
+      by eapply expr_has_ty_subst.
+    - apply SetTy with (fty := fty) (t := t) (σ := subst_ty σ <$> σ0) => //; last first.
+      + rewrite -subst_ty_subst; first by eapply expr_has_ty_subst.
+        apply has_field_bounded in hf => //.
+        destruct hf as (hdef & ht & hfty).
+        apply expr_has_ty_wf in he => //.
+        inv he; simplify_eq.
+        by rewrite H2.
+      + change (ClassT t (subst_ty σ <$> σ0)) with (subst_ty σ (ClassT t σ0)).
+        by eapply expr_has_ty_subst.
+    - rewrite fmap_insert /=.
+      eapply NewTy => //.
+      { inv hwf.
+        econstructor => //; first by rewrite map_length.
+        move => k ty.
+        rewrite list_lookup_fmap.
+        destruct (targs !! k) as [ ty' | ] eqn:hty' => //=.
+        case => <-.
+        apply wf_ty_subst => //.
+        by apply H3 in hty'.
+      }
+      move => f fty arg hfty ha.
+      rewrite -subst_ty_subst.
+      + eapply expr_has_ty_subst => //.
+        by eapply hargs.
+      + apply hf in hfty.
+        apply has_field_bounded in hfty => //.
+        destruct hfty as (hdef & ht & hfty).
+        inv hwf; simplify_eq.
+        by rewrite H2.
+    - rewrite fmap_insert /=.
+      rewrite subst_ty_subst; last first.
+      { apply has_method_from_def in hm => //.
+        destruct hm as (odef & mo & ho & hmo & _ & [σo [hin ->]]).
+        rewrite /subst_mdef /=.
+        rewrite map_Forall_lookup in hmb.
+        apply inherits_using_wf in hin => //.
+        destruct hin as (tdef & ? & ht & ho' & hfo & hlo & htyo); simplify_eq.
+        assert (ho' := ho).
+        apply hmb in ho.
+        apply ho in hmo.
+        destruct hmo as [_ hret].
+        apply bounded_subst with (n := generics odef) => //.
+        apply expr_has_ty_wf in he => //.
+        inv he; simplify_eq.
+        by rewrite H2.
+      }
+      eapply CallTy => //.
+      + change (ClassT t (subst_ty σ <$> targs)) with (subst_ty σ (ClassT t targs)).
+        by eapply expr_has_ty_subst.
+      + move => x ty arg hty ha.
+        rewrite -subst_ty_subst.
+        { eapply expr_has_ty_subst => //.
+          by eapply hargs.
+        }
+        apply has_method_from_def in hm => //.
+        destruct hm as (odef & mo & ho & hmo & _ & [σo [hin ->]]).
+        rewrite map_Forall_lookup in hmb.
+        apply inherits_using_wf in hin => //.
+        destruct hin as (tdef & ? & ht & ho' & hfo & hlo & htyo); simplify_eq.
+        assert (ho' := ho).
+        apply hmb in ho.
+        apply ho in hmo.
+        destruct hmo as [hargs' _].
+        rewrite map_Forall_lookup in hargs'.
+        rewrite /subst_mdef /= in hty.
+        rewrite lookup_fmap_Some in hty.
+        destruct hty as [ty' [ <- hty]].
+        apply hargs' in hty.
+        apply bounded_subst with (n := generics odef) => //.
+        apply expr_has_ty_wf in he => //.
+        inv he; simplify_eq.
+        by rewrite H2.
+    - econstructor; first by apply lty_sub_subst.
+      by apply hi.
+    - eapply CondTagTy.
+      + by rewrite lookup_fmap hin /=.
+      + by apply lty_sub_subst.
+      + rewrite fmap_insert /= in hi.
+        apply hi.
+        apply map_Forall_insert_2 => //.
+        constructor; last by constructor.
+        rewrite map_Forall_lookup in hwf0.
+        by apply hwf0 in hin.
   Qed.
-   *)
 
   Definition subst_local_tys targs (lty: local_tys) : local_tys :=
     (subst_ty targs) <$> lty.
@@ -899,60 +1802,262 @@ Section ProgDef.
     destruct (lty !! k) as [ty | ] eqn:hty => //=.
     rewrite hty.
     apply h in hty.
-    by rewrite subst_gen_targs_is_bounded.
-  Qed.
-
-  Lemma lty_sub_subst lty rty:
-    lty <:< rty →
-    ∀ targs, (subst_local_tys targs lty) <:< (subst_local_tys targs rty).
-  Proof.
-    rewrite /lty_sub => h targs k A.
-    rewrite !lookup_subst_local_tys.
-    destruct (rty !! k) as [ty | ] eqn:hty; last done.
-    move => /= [<-].
-    apply h in hty as [B [-> hsub]].
-    exists (subst_ty targs B); split; first done.
-    by apply subtype_subst.
-  Qed.
-
-  Lemma expr_has_ty_subst lty e ty:
-    expr_has_ty lty e ty →
-    ∀ targs,
-    expr_has_ty (subst_local_tys targs lty) e (subst_ty targs ty).
-  Proof.
-    induction 1 as [ z | b | | op e1 e2 hop h1 hi1 h2 hi2
-      | op e1 e2 hop h1 hi1 h2 hi2 | v ty hv
-      | e s t hs hi hsub ] => targs; try by constructor.
-    - simpl in *; by constructor.
-    - simpl in *; by constructor.
-    - constructor.
-      by rewrite /subst_local_tys lookup_fmap hv.
-    - econstructor; first by apply hi.
-      by apply subtype_subst.
+    by rewrite subst_ty_id.
   Qed.
 
   (* Consider a class C<T0, ..., Tn>,
      method bodies are checked under a generic env = [| T0, .., Tn |]
    *)
-  Definition wf_mdef_ty t n mdef :=
-    let targs := gen_targs n in
-    ∃ lty,
-    cmd_has_ty (<["$this" := ClassT t targs]>(subst_local_tys targs mdef.(methodargs))) mdef.(methodbody) lty ∧
-    expr_has_ty lty mdef.(methodret) (subst_ty targs mdef.(methodrettype))
+  Definition wf_mdef_ty this σ mdef :=
+    ∃ rty,
+    cmd_has_ty (<["$this" := this]>(subst_ty σ <$> mdef.(methodargs))) mdef.(methodbody) rty ∧
+    expr_has_ty rty mdef.(methodret) (subst_ty σ mdef.(methodrettype))
+  .
+
+  Definition cdef_wf_mdef_ty cname cdef :=
+    let σ := gen_targs cdef.(generics) in
+    map_Forall (λ _mname mdef, wf_mdef_ty (ClassT cname σ) σ mdef) cdef.(classmethods)
   .
 
   Record wf_cdefs (prog: stringmap classDef) := {
+    wf_extends_wf : wf_no_cycle prog;
+    wf_parent : map_Forall (λ _cname, wf_cdef_parent prog) prog;
+    wf_override : wf_method_override Δ;
     wf_fields : map_Forall (λ _cname, wf_cdef_fields) prog;
     wf_fields_bounded : map_Forall (λ _cname, wf_cdef_fields_bounded) prog;
-    wf_methods : map_Forall (λ _cname, wf_cdef_methods) prog;
+    wf_fields_wf  : map_Forall (λ _cname, wf_cdef_fields_wf) prog;
     wf_methods_bounded : map_Forall (λ _cname, cdef_methods_bounded) prog;
-    wf_mdefs :
-      map_Forall (λ cname cdef,
-        map_Forall (λ _mname mdef,
-           wf_mdef_ty cname cdef.(generics) mdef)
-        cdef.(classmethods)) prog
+    wf_methods_wf : map_Forall (λ _cname, wf_cdef_methods_wf) prog;
+    wf_mdefs : map_Forall cdef_wf_mdef_ty prog;
   }
   .
+
+  Lemma expr_has_ty_subl lty e ty:  
+    map_Forall (λ _, wf_ty) lty →
+    expr_has_ty lty e ty →
+    ∀ lty', lty' <:< lty →
+    expr_has_ty lty' e ty.
+  Proof.
+    move => hwf.
+    induction 1 as [ z | b | | op e1 e2 hop h1 hi1 h2 hi2 |
+      op e1 e2 hop h1 hi1 h2 hi2 | v ty h | e s t h hi hsub ] => lty' hlty//=; try (by constructor).
+    - constructor; by eauto.
+    - constructor; by eauto.
+    - assert (hh : wf_ty ty) by (by apply hwf in h).
+      apply hlty in h.
+      destruct h as [ty' [ h hsub]].
+      eapply ESubTy => //.
+      by constructor.
+    - apply hi in hlty.
+      by econstructor.
+  Qed.
+
+  Lemma cmd_has_ty_subl lty cmd rty :
+    map_Forall (λ _ : string, wf_cdef_parent Δ) Δ →
+    map_Forall (λ _ : string, wf_ty) lty →
+    cmd_has_ty lty cmd rty →
+    ∀ lty', lty' <:< lty →
+    cmd_has_ty lty' cmd rty.
+  Proof.
+    move => hp hwf.
+    induction 1 as [ lty | ????? h1 hi1 h2 hi2 | ???? he |
+      ????? he h1 hi1 h2 hi2 | ??????? he hf |
+      ??????? he hf hr | ?????? ht hf hdom hargs |
+      ????????? he hm hdom hargs |
+      ???? hsub h hi | ?????? hin hr h hi ] => //= lty' hlty'.
+    - apply SubTy with lty' => //.
+      by constructor.
+    - econstructor; by eauto.
+    - eapply SubTy; first by apply lty_sub_insert_1.
+      constructor.
+      by apply expr_has_ty_subl with lty.
+    - constructor; try (by eauto).
+      by apply expr_has_ty_subl with lty1.
+    - eapply SubTy; first by apply lty_sub_insert_1.
+      econstructor; last done.
+      by apply expr_has_ty_subl with lty.
+    - apply SubTy with lty' => //.
+      econstructor; [| done|]; by eapply expr_has_ty_subl.
+    - eapply SubTy; first by apply lty_sub_insert_1.
+      econstructor => //.
+      move => f fty arg hfty ha.
+      eapply expr_has_ty_subl => //.
+      by eapply hargs.
+    - eapply SubTy; first by apply lty_sub_insert_1.
+      econstructor => //.
+      + by eapply expr_has_ty_subl.
+      + move => f fty arg hfty ha.
+        eapply expr_has_ty_subl => //.
+        by eapply hargs.
+    - econstructor; by eauto.
+    - destruct (hlty' _ _ hin) as [ty' [? ?]].
+      eapply CondTagTy.
+      + done.
+      + by eapply lty_sub_transitive.
+      + eapply hi.
+        * rewrite map_Forall_lookup => x tx.
+          rewrite lookup_insert_Some.
+          case => [[? <-] | [? hx]].
+          { constructor; last by constructor.
+            by apply hwf in hin.
+          }
+          by apply hwf in hx.
+        * eapply lty_sub_transitive; first by apply lty_sub_insert_1.
+          apply lty_sub_insert_2.
+          by eauto.
+  Qed.
+
+  Lemma wf_mdef_ty_inherits t0 t σ m mdef orig def def0:
+    map_Forall (λ _ : string, wf_cdef_parent Δ) Δ →
+    map_Forall (λ _ : string, wf_cdef_fields_wf) Δ →
+    map_Forall (λ _ : string, wf_cdef_methods_wf) Δ →
+    map_Forall (λ _ : string, wf_cdef_fields_bounded) Δ →
+    map_Forall (λ _ : string, cdef_methods_bounded) Δ →
+    Δ !! t = Some def →
+    Δ !! t0 = Some def0 →
+    has_method m t orig mdef →
+    wf_mdef_ty (ClassT t (gen_targs def.(generics))) (gen_targs def.(generics)) mdef →
+    inherits_using t0 t σ →
+    wf_mdef_ty (ClassT t0 (gen_targs def0.(generics))) σ mdef.
+  Proof.
+    move => hp hfwf hmwf hfb hmb hΔt hΔt0 hm [rty [hbody hret]] hin.
+    assert (h: Forall (bounded (generics def0)) σ
+            ∧ length σ = generics def ∧ Forall wf_ty σ).
+    { apply inherits_using_wf in hin => //.
+      destruct hin as (? & ? & ? & ? &? & ? & ?).
+      by simplify_eq.
+    }
+    destruct h as (hF & hL & hσ).
+    apply has_method_from_def in hm => //.
+    destruct hm as (def' & mdef_orig & ho & hmdef_orig & _ & σm & hσm & hmdef).
+    apply inherits_using_wf in hσm => //.
+    destruct hσm as (def'' & odef'' & ? & ? & ? & ? & ? );
+    assert (ho' := ho).
+    assert (hmdef_orig' := hmdef_orig).
+    apply hmwf in ho'.
+    apply ho' in hmdef_orig' as [hargs _].
+    exists (subst_ty σ <$> rty); split.
+    - apply cmd_has_ty_subl with (<["$this":=ClassT t σ]>(subst_ty σ <$> methodargs mdef)) => //.
+      + rewrite map_Forall_lookup => x tx.
+        rewrite lookup_insert_Some.
+        simplify_eq.
+        case => [[? <-]|[? ]].
+        * econstructor => //.
+          rewrite Forall_forall in hσ => k ty hk.
+          apply elem_of_list_lookup_2 in hk.
+          by apply hσ.
+        * rewrite lookup_fmap_Some.
+          case => [ty [<- ]].
+          rewrite /subst_mdef /=.
+          rewrite lookup_fmap_Some.
+          case => [tz [<- hz]].
+          apply wf_ty_subst => //.
+          apply wf_ty_subst => //.
+          by apply hargs in hz.
+      + replace (ClassT t σ) with (subst_ty σ (ClassT t (gen_targs def.(generics)))); last first.
+        { by rewrite /= subst_ty_gen_targs. }
+        replace (<["$this":=subst_ty σ (ClassT t (gen_targs (generics def)))]> (subst_ty σ <$> methodargs mdef))
+          with (subst_ty σ <$> (<["$this" := ClassT t (gen_targs (generics def))]> (methodargs mdef))); last first.
+        { by rewrite fmap_insert. }
+        apply cmd_has_ty_subst => //.
+        * rewrite map_Forall_lookup => x tx.
+          rewrite lookup_insert_Some.
+          simplify_eq.
+          case => [[? <-] | [? ]].
+          { econstructor => //; first by rewrite length_gen_targs. 
+            by apply gen_targs_wf.
+          }
+          rewrite /subst_mdef /=.
+          rewrite lookup_fmap_Some.
+          case => [tz [<- hz]].
+          apply wf_ty_subst => //.
+          by apply hargs in hz.
+        * move: hbody.
+          simplify_eq.
+          rewrite fmap_subst_tys_id => //.
+          rewrite map_Forall_lookup /subst_mdef /= => k tk.
+          rewrite lookup_fmap_Some; case => [ty [<- hty]].
+          eapply bounded_subst => //.
+          apply hmb in ho.
+          apply ho in hmdef_orig.
+          by apply hmdef_orig in hty.
+      + move => x tx.
+        rewrite lookup_insert_Some.
+        case => [[<- <-]|[?]].
+        * rewrite lookup_insert.
+          eexists; split => //.
+          replace σ with (subst_ty (gen_targs def0.(generics)) <$> σ); last first.
+          { by rewrite subst_tys_id. }
+          eapply subtype_inherits_using => //.
+          by rewrite length_gen_targs.
+        * rewrite lookup_fmap_Some.
+          case => [ty [<- hx]].
+          rewrite lookup_insert_ne // lookup_fmap hx /=.
+          by eexists.
+    - apply expr_has_ty_subst => //.
+      replace (methodrettype mdef) with (subst_ty (gen_targs (generics def)) (methodrettype mdef)); first done.
+      simplify_eq.
+      rewrite subst_ty_id // /subst_mdef /=.
+      eapply bounded_subst => //.
+      apply hmb in ho.
+      apply ho in hmdef_orig.
+      by apply hmdef_orig.
+  Qed.
+          
+  Lemma has_method_wt lty recv t σ name orig mdef:
+    map_Forall (λ _ : string, wf_cdef_parent Δ) Δ →
+    map_Forall (λ _ : string, wf_cdef_fields_wf) Δ →
+    map_Forall (λ _ : string, wf_cdef_fields_bounded) Δ →
+    map_Forall (λ _ : string, cdef_methods_bounded) Δ →
+    map_Forall (λ _cname, wf_cdef_methods_wf) Δ →
+    map_Forall cdef_wf_mdef_ty Δ →
+    map_Forall (λ _ : string, wf_ty) lty →
+    expr_has_ty lty recv (ClassT t σ) →
+    has_method name t orig mdef →
+    ∃ rty,
+    cmd_has_ty (<["$this" := ClassT t σ]>(subst_ty σ <$> mdef.(methodargs))) mdef.(methodbody) rty ∧
+    expr_has_ty rty mdef.(methodret) (subst_ty σ mdef.(methodrettype)).
+  Proof.
+    move => hp hfwf hfb hmb hmwf hwf hlty hrecv hhm.
+    assert (hhm' := hhm).
+    apply has_method_from_def in hhm' => //.
+    destruct hhm' as (odef & omdef & hodef & homdef & hm & [σ0 [hin ->]]).
+    assert (hdef: is_Some (Δ !! t)).
+    { apply inherits_using_wf in hin => //.
+      by destruct hin as (? & ? & -> & _).
+    }
+    destruct hdef as [def hdef].
+    destruct (wf_mdef_ty_inherits t orig σ0 name omdef orig odef def) as [rty [hbody hret]] => //.
+    { apply hwf in hodef.
+      by apply hodef in homdef.
+    }
+    apply expr_has_ty_wf in hrecv => //.
+    exists (subst_ty σ <$> rty); split.
+    - replace (ClassT t σ) with (subst_ty σ (ClassT t (gen_targs def.(generics)))); last first.
+      { rewrite /= subst_ty_gen_targs //.
+        inv hrecv.
+        by simplify_eq.
+      }
+      rewrite -fmap_insert.
+      apply wf_ty_class_inv in hrecv.
+      apply cmd_has_ty_subst => //.
+      rewrite map_Forall_lookup => x tx.
+      rewrite lookup_insert_Some.
+      case => [[? <-]|[? ]].
+      * econstructor => //; first by rewrite length_gen_targs.
+        by apply gen_targs_wf.
+      * rewrite /subst_mdef /= lookup_fmap_Some.
+        case => [ty [<- hx]].
+        apply wf_ty_subst.
+        { apply inherits_using_wf in hin => //.
+          by repeat destruct hin as [? hin].
+        }
+        apply hmwf in hodef.
+        apply hodef in homdef.
+        by apply homdef in hx.
+    - apply expr_has_ty_subst => //.
+      by apply wf_ty_class_inv in hrecv.
+  Qed.
 
   (* Big step reduction *)
   Definition primop_eval (op: primop) : Z → Z → value :=
@@ -1096,12 +2201,12 @@ Section ProgDef.
         expr_eval st1.1 cond = Some (BoolV false) →
         cmd_eval st1 els st2 n →
         cmd_eval st1 (IfC cond thn els) st2 n
-    | CallEv: ∀ le h h' lhs recv l t vs name args vargs mdef
+    | CallEv: ∀ le h h' lhs recv l t vs name args vargs orig mdef
         run_env run_env' ret n,
         expr_eval le recv = Some (LocV l) →
         map_args (expr_eval le) args = Some vargs →
         h !! l = Some (t, vs) →
-        has_method name mdef t →
+        has_method name t orig mdef →
         <["$this" := LocV l]>vargs = run_env →
         cmd_eval (run_env, h) mdef.(methodbody) (run_env', h') n →
         expr_eval run_env' mdef.(methodret) = Some ret →
