theories/adequacy.v
@@ -12,8 +12,6 @@ From iris.proofmode Require Import tactics.
 
 From shack Require Import lang heap modality interp.
 
-Check fmap.
-
 Section proofs.
   (* assume a given set of class definitions *)
   Context `{PDC: ProgDefContext}.
@@ -65,15 +63,17 @@ Section proofs.
 
   Lemma expr_adequacy (σi:interp_env) e lty le ty val :
     map_Forall (λ _cname, wf_cdef_fields) Δ →
+    map_Forall (λ _cname, wf_cdef_fields_bounded) Δ →
+    map_Forall (λ _cname, wf_cdef_parent Δ) Δ →
     expr_eval le e = Some val →
     expr_has_ty lty e ty →
     interp_local_tys σi lty le -∗
     interp_type ty σi val.
   Proof.
-    move => hwf he h; move: le val he.
+    move => ??? he h; move: le val he.
     elim: h => [z | b | | op e1 e2 hop he1 hi1 he2 hi2 |
         op e1 e2 hop he1 hi1 he2 hi2 |
-        v vty hv | exp S T hS hi hsub ] le val he; iIntros "#Hlty".
+        v vty hv | exp S T hS hi hwf hsub ] =>  le val he; iIntros "#Hlty".
     - inv he; rewrite interp_type_unfold /=; by eauto.
     - inv he; rewrite interp_type_unfold /=; by eauto.
     - inv he; rewrite interp_type_unfold /=; by eauto.
@@ -131,6 +131,8 @@ Section proofs.
 
   Lemma interp_local_tys_weaken_ty (σi: interp_env) v A B lty lty' le:
     map_Forall (λ _cname, wf_cdef_fields) Δ →
+    map_Forall (λ _cname, wf_cdef_fields_bounded) Δ →
+    map_Forall (λ _cname, wf_cdef_parent Δ) Δ →
     lty !! v = Some A →
     lty' !! v = Some B →
     (∀ w, v ≠ w → lty !! w = lty' !! w) →
@@ -138,7 +140,7 @@ Section proofs.
     interp_local_tys σi lty le -∗
     interp_local_tys σi lty' le.
   Proof.
-    move => hwf hin1 hin2 hs hAB; iIntros "H".
+    move => ??? hin1 hin2 hs hAB; iIntros "H".
     rewrite /interp_local_tys.
     iIntros (w ty) "%Hin".
     destruct (decide (v = w)) as [<- | hne].
@@ -168,6 +170,8 @@ Section proofs.
 
   Lemma interp_local_tys_list (σi:interp_env) lty le targs args vargs:
     map_Forall (λ _cname, wf_cdef_fields) Δ →
+    map_Forall (λ _cname, wf_cdef_fields_bounded) Δ →
+    map_Forall (λ _cname, wf_cdef_parent Δ) Δ →
     dom stringset targs = dom stringset args →
     map_args (expr_eval le) args = Some vargs →
     (∀ (x : string) (ty : lang_ty) (arg : expr),
@@ -177,7 +181,7 @@ Section proofs.
     interp_local_tys σi lty le -∗
     interp_local_tys σi targs vargs.
   Proof.
-    move => hwf hdom hargs helt.
+    move => ??? hdom hargs helt.
     iIntros "#Hle" (v ty) "%hin".
     assert (ha: ∃ arg, args !! v = Some arg).
     { apply elem_of_dom.
@@ -213,9 +217,9 @@ Section proofs.
     iDestruct "hmodels" as (sh) "[hown [%hdom #h]]".
     iExists sh.
     rewrite interp_class_unfold.
-    iDestruct "hrecv" as (l' t' fields ifields) "[%H [hsem hl]]".
-    iDestruct "hsem" as "[%hdomf #hifields]".
-    destruct H as [[= <-] [ hinherits' hfields]].
+    iDestruct "hrecv" as (l' t' σ' σt' fields ifields) "[%H [hsem_d [hsem_s hl]]]".
+    iDestruct "hsem_s" as "[%hdomf #hifields]".
+    destruct H as [[= <-] [ hinherits' [hwfσ' [hσ' hfields]]]].
     iDestruct (sem_heap_own_valid_2 with "hown hl") as "#Hv".
     iSplitL; first by iFrame.
     iSplitR.
@@ -259,179 +263,43 @@ Section proofs.
       by iPureIntro.
   Qed.
 
-  (* Lemma interp_mixed_spec σi v: *)
-  (*   map_Forall (fun _ => wf_cdef_fields) Δ → *)
-  (*   interp_type MixedT σi v -∗ *)
-  (*   (interp_int v ∨ interp_bool v ∨ interp_null v ∨ *)
-  (*   ∃ l t ifields, ⌜v = LocV l⌝ ∧ l ↦ (t, ifields) ∧ interp_ex σi t interp_type v)%I. *)
-  (* Proof. *)
-  (*   move => hwf. *)
-  (*   rewrite interp_type_unfold /=. *)
-  (*   iIntros "[H | H]"; last first. *)
-  (*   { by iRight; iRight; iLeft. } *)
-  (*   iDestruct "H" as "[? | H]". *)
-  (*   { by iLeft. } *)
-  (*   iDestruct "H" as "[? | H]". *)
-  (*   { by iRight; iLeft. } *)
-  (*   iDestruct "H" as (t σt l rt fields ifields) "[%Heq [#Hfields #hl]]". *)
-  (*   destruct Heq as [-> [hinherits hrtf]]. *)
-  (*   iRight; iRight; iRight. *)
-  (*   iExists l, rt, ifields. *)
-  (*   iSplit; first done. *)
-  (*   iSplit; first done. *)
-  (*   iDestruct "Hfields" as "[%hdom #Hfields]". *)
-    
-  (*   apply inherits_to_using in hinherits. *)
-  (*   destruct hinherits as [-> | [σin hinherits]]; last first. *)
-  (*   - iExists (subst_ty σin <$> σt), l, rt, fields, ifields. *)
-  (*     iSplit; first done. *)
-  (*     iSplit; last done. *)
-  (*     iSplit; first done. *)
-  (*     iIntros (f ty) "%hf". *)
-  (*     assert (hf': has_field f t (subst_ty σin ty)). *)
-  (*      eapply has_field_inherits => //. *)
-
-  (* Lemma inherits_to_using A B: *)
-  (*   inherits A B → (A = B) ∨ ∃ σ, inherits_using A B σ. *)
-
-(* Lemma has_field_inherits : *)
-  (* map_Forall (fun _ => wf_cdef_fields) Δ → *)
-  (* ∀ A B σ, inherits_using A B σ → *) 
-  (* ∀ f fty, has_field f B fty → has_field f A (subst_ty σ fty). *)
-  (*
-  Lemma interp_class_loc_inversion σi h l C σC t fields:
-    h !! l = Some (t, fields) →
-    heap_models h -∗
-    interp_class C σC σi interp_type (LocV l) -∗
-    heap_models h ∗ interp_type (ExT t) σi (LocV l).
-  Proof.
-    move => hl; iIntros "Hh H".
-    iDestruct "H" as (????) "[%H [#Hifields H◯]]".
-    destruct H as [[= <-] [hinherits hfields]].
-    rewrite /interp_ex interp_type_unfold /=.
-    iDestruct "Hh" as (sh) "[hown [%hdom #h]]".
-    iDestruct (sem_heap_own_valid_2 with "hown H◯") as "#Hv".
-    iSplitL "hown".
-    { iExists _; iSplitL; first done.
-      by iSplit.
-    }
-    iSpecialize ("h" $! l t fields hl).
-    iDestruct "h" as (iFs) "[HiFs hmodfs]".
-    iRewrite "HiFs" in "Hv".
-    rewrite !option_equivI prod_equivI /=.
-    iDestruct "Hv" as "[%ht #heq]".
-    fold_leibniz; subst.
-    iExists σC, l, t0, fields0, ifields.
-    iSplitR; first done.
-    iSplitR; last done.
-    iDestruct "Hifields" as "[%hfdom #Hifields]".
-    iSplit; first done.
-
-
-
-
-
-
-    iDestruct ((heap_models_class _ _ cname _ _ hl) with "[Hh //]") as "Hv".
-    iApply "Hv".
-    by rewrite interp_type_unfold.
-  Qed.
-
-  Lemma interp_nonnull_loc_inversion σi h (v: string) l t fields:
-    h !! l = Some (t, fields) →
-    heap_models h -∗
-    interp_nonnull σi interp_type (LocV l) -∗
-    heap_models h ∗ interp_type (ExT t) σi (LocV l).
-  Proof.
-    move => hl; iIntros "Hh H".
-    iDestruct "H" as "[H | H]".
-    { iDestruct "H" as (z) "%H"; discriminate. }
-    iDestruct "H" as "[H | H]".
-    { iDestruct "H" as (b) "%H"; discriminate. }
-    iDestruct "H" as (cname) "H".
-    iFrame.
-    rewrite interp_type_unfold.
-    by iApply ((interp_class_loc_inversion _ v _ cname) with "[Hh]").
-  Qed.
-
-  Lemma interp_type_loc_inversion σi h le lty (v: string) l T t fields:
-    h !! l = Some (t, fields) →
-    le !! v = Some (LocV l) →
-    interp_local_tys σi lty le -∗
-    heap_models h -∗
-    interp_type T σi (LocV l) -∗
-    heap_models h ∗ interp_type (ExT t) σi (LocV l).
-  Proof.
-    rewrite interp_type_unfold => hl hv;  elim: T v hv => /=.
-    - move => ??; iIntros "? ? H".
-      iDestruct "H" as (z) "%H"; discriminate.
-    - move => ??; iIntros "? ? H".
-      iDestruct "H" as (b) "%H"; discriminate.
-    - move => ??; iIntros "? ? H".
-      iDestruct "H" as "%H"; by elim H.
-    - move => v hv; iIntros "#Hs Hh H".
-      iDestruct "H" as "[H | H]"; last first.
-      { iDestruct "H" as "%H"; discriminate. }
-      by iApply ((interp_nonnull_loc_inversion _ v) with "[Hh]").
-    - move => cname v hv; iIntros "Hs Hh H".
-      by iApply ((interp_class_loc_inversion _ v _ cname) with "[Hh]").
-    - move => ??; iIntros "? ? H".
-      iDestruct "H" as "%H"; discriminate.
-    - move => v hv; iIntros "#Hs Hh H".
-      by iApply ((interp_nonnull_loc_inversion _ v) with "[Hh]").
-    - move => S hS T hT v hv; iIntros "#Hs Hh H".
-      iDestruct "H" as "[H | H]".
-      + apply hS in hv.
-        by iApply (hv with "Hs Hh H").
-      + apply hT in hv.
-        by iApply (hv with "Hs Hh H").
-    - move => S hS T hT v hv; iIntros "#Hs Hh H".
-      iAssert (interp_type S (LocV l)) with "[H]" as "hs".
-      { rewrite interp_type_unfold.
-        by iDestruct "H" as "[HS HT]".
-      }
-      apply hS in hv.
-      rewrite -!interp_type_unfold in hv.
-      by iApply (hv with "Hs Hh hs").
-  Qed.
-   *)
-
   Lemma cmd_adequacy_ lty cmd lty' :
     wf_cdefs Δ →
+    map_Forall (λ _, wf_ty) lty →
     ⌜cmd_has_ty lty cmd lty'⌝ -∗
     ∀ (σi: interp_env) st st' n, ⌜cmd_eval st cmd st' n⌝ -∗
     heap_models st.2 ∗ interp_local_tys σi lty st.1 -∗ |=▷^n
         heap_models st'.2 ∗ interp_local_tys σi lty' st'.1.
   Proof.
-    move => wfΔ.
-    iLöb as "IH" forall (lty cmd lty').
-    (* iIntros (wftys). *)
+    move => wfΔ wflty.
+    iLöb as "IH" forall (lty cmd lty' wflty).
     iIntros "%hty" (σi st st' n) "%hc".
     iInduction hty as [ lty | lty1 lty2 lty3 fstc sndc hfst hi1 hsnd hi2 |
         lty lhs e ty he | lty1 lty2 cond thn els hcond hthn hi1 hels hi2 |
         lty lhs recv t targs name fty hrecv hf |
         lty recv fld rhs fty t σ hrecv hrhs hf |
-        lty lhs t targs args fields (*cdef hΔ hconstraints*) hf hdom harg |
-        (* lty lhs recv t targs name mdef args hrecv hm hdom hi | *)
+        lty lhs t targs args fields hwf hf hdom harg |
+        lty lhs recv t targs name orig mdef args hrecv hfrom hdom hi |
         lty c rty' rty hsub h hi |
-        lty v tv t cmd hv h hi
+        lty rty v tv t cmd hv hr h hi
       ] "IHty" forall (st st' n hc).
     - (* SkipC *) inv hc.
       rewrite updN_zero.
       by iIntros "?".
     - (* SeqC *) inv hc. iIntros "H".
-      iSpecialize ("IHty" with "[//] H").
+      iSpecialize ("IHty" $! wflty with "[//] H").
       rewrite Nat_iter_add.
       iApply (updN_mono_I with "[] IHty").
-      by iApply "IHty1".
+      iApply "IHty1" => //.
+      destruct wfΔ.
+      by apply cmd_has_ty_wf in hfst.
     - (* LetC *)
       inv hc.
       iClear "IH".
       iIntros "[? #Hle]".
       rewrite updN_zero /=.
       iFrame.
-      iDestruct (expr_adequacy with "Hle") as "#?" => //.
-      { by apply wfΔ. }
+      iDestruct (expr_adequacy with "Hle") as "#?" => //; try (by apply wfΔ).
       by iApply interp_local_tys_update.
     - (* IfC *) inv hc
       + iIntros "H". by iApply "IHty".
@@ -440,11 +308,10 @@ Section proofs.
       iClear "IH".
       iIntros "[Hh #Hle]".
       iModIntro. (* keep the later *)
-      iDestruct (expr_adequacy with "Hle") as "#He" => //.
-      { by apply wfΔ. }
+      iDestruct (expr_adequacy with "Hle") as "#He" => //; try (by apply wfΔ).
       rewrite interp_class_unfold /=.
-      iDestruct "He" as (????) "[%H [#Hifields H◯]]".
-      destruct H as [[= <-] [hinherits hfields]].
+      iDestruct "He" as (??????) "[%H [_ [#Hifields H◯]]]".
+      destruct H as [[= <-] [hinherits [_ hfields]]].
       iAssert (heap_models h ∗ ▷ interp_type (subst_ty targs fty) σi v)%I with "[Hh]" as "[Hh Hv]".
       { iDestruct "Hh" as (sh) "(H● & %hdom & #Hh)".
         iDestruct (sem_heap_own_valid_2 with "H● H◯") as "#HΦ".
@@ -461,7 +328,7 @@ Section proofs.
         iRewrite -"HΦ" in "Hifields".
         iSpecialize ("h" $! name _ with "[Hifields]"); first done.
         iDestruct "h" as (w) "[%hw hiw]".
-        by rw_inj hw H7.
+        by simplify_eq.
       }
       iNext.
       iFrame.
@@ -471,13 +338,11 @@ Section proofs.
       iIntros "[Hh #Hle]" => /=.
       iSplitL; last done.
       iApply heap_models_update => //.
-      + iApply expr_adequacy => //.
-        by apply wfΔ.
-      + iApply expr_adequacy => //.
-        by apply wfΔ.
+      + iApply expr_adequacy => //; by apply wfΔ.
+      + iApply expr_adequacy => //; by apply wfΔ.
     - (* NewC *) inv hc.
       iIntros "[Hh #Hle]"; simpl.
-      (* we need one modality to update the semantic heap *)
+      (* we need one modality to emantic heap *)
       iDestruct "Hh" as (sh) "(H● & %Hdom & #Hh)".
       assert (hnew: sh !! new = None).
       { apply (not_elem_of_dom (D:=gset loc)).
@@ -490,204 +355,367 @@ Section proofs.
         first by apply (sem_heap_view_alloc _ new t iFs).
       iIntros "!> !>". (* kill the modalities *)
       iAssert (interp_type (ClassT t targs) σi (LocV new)) with "[]" as "#Hl".
-      { rewrite interp_type_unfold /=.
-        iExists _, _, _, _.
-        iSplit; first done.
-        iSplit; last done.
-        rewrite /interp_fields; iSplit; first by rewrite /iFs !dom_fmap_L.
-        iIntros (f fty) "%hfty".
-        rewrite /iFs !lookup_fmap.
-        apply hf in hfty.
-        by rewrite hfty /=.
+      {
+        iAssert (interp_fields σi t targs fields iFs interp_type) as "HiFs".
+        { rewrite /interp_fields; iSplit; first by rewrite /iFs !dom_fmap_L.
+          iIntros (f fty) "%hfty".
+          apply hf in hfty.
+          rewrite /iFs !lookup_fmap.
+          by rewrite hfty /=.
+        }
+        rewrite interp_type_unfold /=.
+        assert (hwf' := hwf).
+        inv hwf'.
+        iExists new, t, (gen_targs def.(generics)), targs, fields, iFs.
+        iSplit; last by (repeat iSplit => //).
+        iPureIntro.
+        repeat split => //.
+        + by econstructor.
+        + by rewrite subst_ty_gen_targs.
       }
       iSplitL; last by iApply interp_local_tys_update.
       iExists _. iFrame. iSplit; first by rewrite !dom_insert_L Hdom.
       iModIntro. iIntros (???) "Hlook".
       rewrite lookup_insert_Some.
-      iDestruct "Hlook" as %[[<- [= <- <-]]|[Hℓ Hlook]].
-      + iExists _. rewrite lookup_insert.
-        iSplitR; first done.
-        rewrite /heap_models_fields.
-        iSplitR.
-        {
-          apply dom_map_args in H6.
-          by rewrite /iFs !dom_fmap_L H6 -hdom.
-        }
-        iIntros (f iF) "hiF".
-        iAssert (⌜f ∈ dom stringset fields⌝)%I as "%hfield".
-        {
-          rewrite !lookup_fmap.
-          rewrite elem_of_dom.
-          destruct (fields !! f) => //=.
-          by rewrite option_equivI.
-        }
-        assert (h0: is_Some (args !! f)).
-        {
-          apply elem_of_dom.
-          by rewrite -hdom.
-        }
-        destruct h0 as [a0 ha0].
-        assert (h1: is_Some (vargs !! f)).
-        {
-          apply elem_of_dom.
-          apply dom_map_args in H6.
-          by rewrite H6 -hdom.
-        }
-        destruct h1 as [v0 hv0].
-        assert (h2: is_Some (fields !! f)) by (by apply elem_of_dom).
-        destruct h2 as [fty hty].
-        iExists v0; iSplitR; first done.
-        rewrite /interp_fields lookup_fmap.
-        assert (heval0: expr_eval le a0 = Some v0).
-        { rewrite (map_args_lookup _ _ _ args vargs H6 f) in hv0.
-          by rewrite ha0 in hv0.
-        }
-        assert (hty0: expr_has_ty lty a0 (subst_ty targs fty)) by (by apply harg with f).
-        rewrite !lookup_fmap hty /=  option_equivI later_equivI.
-        iNext.
-        rewrite discrete_fun_equivI.
-        iSpecialize ("hiF" $! v0).
-        iRewrite -"hiF".
-        iDestruct (expr_adequacy _ a0 with "Hle") as "#Ha0" => //.
-        by apply wfΔ.
-      + rewrite lookup_insert_ne; last done.
+      iDestruct "Hlook" as %[[<- [= <- <-]]|[Hℓ Hlook]]; last first.
+      { rewrite lookup_insert_ne; last done.
         by iApply "Hh".
-        (*
-    - (* CallC *) inv hc. iIntros "[Hh #Hle]".
-      assert (wfbody: ∃B cdef,
-        Δ !! B = Some cdef ∧
-        wf_mdef_ty B cdef.(generics) mdef0 ∧
-        wf_mdef_bounded cdef.(generics) mdef0 ∧
-        inherits t0 B).
-      { destruct wfΔ as [_ _ _ hbounded hbodies].
-        rewrite map_Forall_lookup in hbodies.
-        rewrite map_Forall_lookup in hbounded.
-        admit (*
-        apply has_method_from in H7.
-        destruct H7 as (B & cdef & hΔB & heq & hin).
-        assert (hbody := hΔB).
-        assert (hbound := hΔB).
-        apply hbodies in hbody.
-        apply hbounded in hbound.
-        rewrite map_Forall_lookup in hbody.
-        exists B; exists cdef; split; first done.
-        split; last split; last done.
-        + by apply hbody in heq.
-        + by apply hbound in heq.
-               *).
       }
-      destruct wfbody as (B & cdef & hΔB & wfbody & wfbounded & hinherits).
-      destruct wfbody  as (lty_body & hbody & hret).
-      iAssert(⌜inherits t0 t⌝ ∗ interp_type (ClassT B targs) env (LocV l))%I as "#Hl".
-      { iDestruct (expr_adequacy _ recv with "Hle") as "#Hrecv" => //.
-        rewrite !interp_type_unfold /= /interp_class.
-        iDestruct "Hrecv" as (? t1 ?) "[%hpure Hsem]".
-        destruct hpure as [[= <-] [hinherits' ?]].
-        iDestruct "Hh" as (sh) "(H● & % & #Hh)".
-        iDestruct (sem_heap_own_valid_2 with "H● Hsem") as "#HΦ".
-        iDestruct ("Hh" with "[//]") as (?) "[H H▷]".
-        iRewrite "H" in "HΦ".
-        rewrite option_equivI prod_equivI /=.
-        iDestruct "HΦ" as "[%Ht HΦ]".
-        fold_leibniz; rewrite Ht.
-        iSplitR; first done.
-        iExists l, t1, fields; iSplitR; last done.
-        iPureIntro; split; first done.
-        split => //.
-        by rewrite -Ht.
-      }
-      iDestruct "Hl" as "[%Hinherits #Hl]".
-      assert (hincl: mdef_incl mdef0 mdef).
+      iExists _. rewrite lookup_insert.
+      iSplitR; first done.
+      rewrite /heap_models_fields.
+      iSplitR.
       {
-        eapply has_method_inherits in Hinherits; [ | by apply wfΔ | done ].
-        destruct Hinherits as [? [? ?]].
-        replace x with mdef0 in * by (by eapply has_method_fun).
-        done.
+        apply dom_map_args in H6.
+        by rewrite /iFs !dom_fmap_L H6 -hdom.
       }
-      (*
-      assert (hbody':
-        cmd_has_ty
-          (<["$this":=ClassT B targs]> (subst_local_tys targs (methodargs mdef0)))
-          (methodbody mdef0)
-          (subst_local_tys targs lty_body)).
-      { replace (ClassT B targs) with
-         (subst_ty targs (ClassT B (gen_targs (generics cdef)))).
-        + rewrite -insert_subst_local_tys.
-          apply cmd_has_ty_subst.
-          rewrite subst_local_tys_gen_targs_is_bounded // in hbody.
-          by apply wfbounded.
-        +
-          rewrite /= -/fmap gen_targs_map_subst //.
-          admit (* global invariant about targs' length *).
+      iIntros (f iF) "hiF".
+      iAssert (⌜f ∈ dom stringset fields⌝)%I as "%hfield".
+      {
+        rewrite !lookup_fmap.
+        rewrite elem_of_dom.
+        destruct (fields !! f) => //=.
+        by rewrite option_equivI.
       }
-      assert (hret' :
-        expr_has_ty
-          (subst_local_tys targs lty_body)
-          (methodret mdef0)
-          (subst_ty targs (methodrettype mdef0))).
-      { destruct wfbounded as [_ retbounded].
-        rewrite subst_gen_targs_is_bounded // in hret.
-        by apply expr_has_ty_subst.
+      assert (h0: is_Some (args !! f)).
+      {
+        apply elem_of_dom.
+        by rewrite -hdom.
       }
-       *)
-      simpl.
-      iModIntro; iNext.
-      assert (hhh : ∃ env0: interp_env, interp_env_car env0 = (λ ty, interp_type ty env) <$> targs) by admit.
-      destruct hhh as [env0 henv0].
-      iSpecialize ("IH" $! _ _ _ hbody env0 _ _ _ H14); simpl.
-      iDestruct ("IH" with "[Hh Hle]") as "H".
-      { iFrame.
-        iApply interp_local_tys_update => //.
-        + iApply interp_local_tys_list => //.
-          (* first by *)
-          destruct hincl as [? _]; rewrite dom_subst_local_tys -H0 //.
-          move => x ty arg hx harg.
-          destruct hincl as [hdom' [hincl _]].
-          destruct (methodargs mdef !! x) as [ty' | ] eqn:hty'.
-          { apply lookup_subst_local_tys_Some in hx as [ z [ h0 ->]].
-            apply (H1 _ _ _ hty') in harg.
-            econstructor; first by apply harg.
-            apply subtype_subst.
-            by eapply hincl.
+      destruct h0 as [a0 ha0].
+      assert (h1: is_Some (vargs !! f)).
+      {
+        apply elem_of_dom.
+        apply dom_map_args in H6.
+        by rewrite H6 -hdom.
+      }
+      destruct h1 as [v0 hv0].
+      assert (h2: is_Some (fields !! f)) by (by apply elem_of_dom).
+      destruct h2 as [fty hty].
+      iExists v0; iSplitR; first done.
+      rewrite /interp_fields lookup_fmap.
+      assert (heval0: expr_eval le a0 = Some v0).
+      { rewrite (map_args_lookup _ _ _ args vargs H6 f) in hv0.
+        by rewrite ha0 in hv0.
+      }
+      assert (hty0: expr_has_ty lty a0 (subst_ty targs fty)) by (by apply harg with f).
+      rewrite !lookup_fmap hty /=  option_equivI later_equivI.
+      iNext.
+      rewrite discrete_fun_equivI.
+      iSpecialize ("hiF" $! v0).
+      iRewrite -"hiF".
+      iDestruct (expr_adequacy _ a0 with "Hle") as "#Ha0" => //; by apply wfΔ.
+    - (* CallC *) inv hc; simpl.
+      destruct wfΔ.
+    
+      (* Get inherits relation between dynamic tag and static tag *)
+      iIntros "[Hh #Hle]".
+      iDestruct (expr_adequacy _ recv with "Hle") as "#Hrecv" => //.
+      rewrite interp_class_unfold /=.
+      iDestruct "Hrecv" as (? ? σin σt fields ifields) "[%Hpure [hifields_d [hifields_s Hl]]]".
+      destruct Hpure as [[= <-] [hσin [hwfσt [htargs hfields]]]].
+      iDestruct "Hh" as (sh) "(H● & %Hdom & #Hh)".
+      iDestruct (sem_heap_own_valid_2 with "H● Hl") as "#HΦ".
+      iDestruct ("Hh" with "[//]") as (?) "[H H▷]".
+      iRewrite "H" in "HΦ".
+      rewrite option_equivI prod_equivI /=.
+      iDestruct "HΦ" as "[%Ht HΦ]".
+      fold_leibniz; subst.
+
+      assert (ht1: is_Some (Δ !! t1)).
+      { apply has_method_from_def in H7 as (? & ? & ? & ? & _ & [? [hin ?]]) => //.
+        by apply inherits_using_wf in hin as (? & ? & ht1 & _).
+      }
+
+      assert (ht : is_Some (Δ !! t)).
+      { apply inherits_using_wf in hσin => //.
+        by destruct hσin as (? & ? & _ & -> & _).
+      }
+      destruct ht as [ def ht ].
+
+      destruct ht1 as [ def1 ht1 ].
+
+      (* Get method inclusion information between mdef0 and mdef *)
+      destruct (has_method_ordered _ _ _ _ _ _ _ _
+        wf_extends_wf wf_override wf_parent wf_methods_bounded
+        hσin H7 hfrom)
+      as (σmin & σot1 & σot & odef0 & odef & omdef0 & omdef &
+         hσeq & ho1 & ho & hom1 & hom & hino & hin1 & hin &
+         _ & ? & heq0 & heq1 & hincl0 & hincl1).
+
+      (* Getting body/ret of static method is well typed *)
+      (* assert (hrecv' := hrecv). *)
+      (* apply has_method_wt with (name0 := name) (orig1 := orig) (mdef1 := mdef) in hrecv' => //. *)
+      (* destruct hrecv' as [rty [hbody hret]]. *)
+
+      (* Get location of the definition of the dynamic method mdef0 *)
+      destruct (has_method_from_def _ _ _ _  wf_parent wf_methods_bounded H7) as
+        (odef0' & mdef0_orig & ho0 & hm0 & hmorig0 & [σ0 [hin0 ->]]).
+      rewrite ho0 in ho1; injection ho1; intros; subst; clear ho1.
+      rewrite subst_mdef_body in H11.
+      rewrite subst_mdef_ret in H12.
+
+      (* Get some type info about dynamic method mdef0 *)
+      assert (hwf0 := hin0).
+      eapply wf_mdef_ty_inherits in hwf0 => //; last first.
+      { apply wf_mdefs in ho0.
+        by apply ho0 in hm0.
+      }
+      
+      (* Random helpers *)
+      assert (bounded (length σ0) (methodrettype mdef0_orig)).
+      { assert (ho0' := ho0).
+        apply wf_methods_bounded in ho0'.
+        apply ho0' in hm0.
+        destruct hm0 as [_ hret].
+        apply inherits_using_wf in hin0 => //.
+        repeat destruct hin0 as [? hin0]; simplify_eq.
+        by rewrite H6.
+      }
+      assert (map_Forall (λ _ : string, bounded (length σ0)) (methodargs mdef0_orig)).
+      { assert (ho0' := ho0).
+        apply wf_methods_bounded in ho0'.
+        apply ho0' in hm0.
+        destruct hm0 as [hargs _].
+        rewrite map_Forall_lookup => k tk hk.
+        apply hargs in hk.
+        apply inherits_using_wf in hin0 => //.
+        repeat destruct hin0 as [? hin0]; simplify_eq.
+        by rewrite H8.
+      }
+      assert (map_Forall (λ _ : string, bounded (length σot)) (methodargs omdef)).
+      { assert (ho' := ho).
+        apply wf_methods_bounded in ho'.
+        apply ho' in hom.
+        destruct hom as [hargs _].
+        rewrite map_Forall_lookup => k tk hk.
+        apply hargs in hk.
+        apply inherits_using_wf in hin => //.
+        repeat destruct hin as [? hin]; simplify_eq.
+        by rewrite H9.
+      }
+      assert (length σt = generics def1).
+      { inv hwfσt.
+        by simplify_eq.
+      }
+
+      assert (Forall wf_ty σt) by (by apply wf_ty_class_inv in hwfσt).
+      assert (hwfot1: Forall wf_ty σot1).
+      { apply inherits_using_wf in hin1 => //.
+        by repeat destruct hin1 as [? hin1].
+      }
+
+      (* add runtime type args into the mix *)
+      assert (hwf1: wf_mdef_ty (ClassT t1 σt) (subst_ty σt <$> σ0) mdef0_orig).
+      { destruct hwf0 as [rty0 [hbody0 hret0]].
+        exists (subst_ty σt <$> rty0); split; last first.
+        + rewrite -subst_ty_subst //.
+          by apply expr_has_ty_subst.
+        + replace (ClassT t1 σt) with (subst_ty σt (ClassT t1 (gen_targs (generics def1)))); last first.
+          { simpl.
+            by rewrite subst_ty_gen_targs.
           }
-        apply mk_is_Some in hx.
-        apply elem_of_dom in hx.
-        rewrite dom_subst_local_tys hdom' in hx.
-        apply elem_of_dom in hx.
-        rewrite hty' in hx.
-        by elim: hx.
+          rewrite -fmap_subst_ty_subst // -fmap_insert.
+          apply cmd_has_ty_subst => //.
+          rewrite map_Forall_lookup => k tk.
+          rewrite lookup_insert_Some.
+          case => [[? <-]|[?]].
+          * econstructor => //; first by rewrite length_gen_targs.
+            by apply gen_targs_wf.
+          * rewrite lookup_fmap_Some.
+            case => [tx [<- hk]].
+            apply wf_ty_subst.
+            { apply inherits_using_wf in hin0 => //.
+              by repeat destruct hin0 as [? hin0].
+            }
+            apply has_method_wf in hmorig0 as [hargs _] => //.
+            by apply hargs in hk.
       }
-      iRevert "H".
+      destruct hwf1 as [rty1 [hbody1 hret1]].
+
+      rewrite hm0 in hom1; injection hom1; intros; subst; clear hom1.
+      replace σ0 with σot1 in *; last by eapply inherits_using_fun.
+      clear hin0.
+
+      assert (wfbody:
+        map_Forall (λ _ : string, wf_ty)
+          (<["$this":=ClassT t1 σt]> (subst_ty (subst_ty σt <$> σot1) <$> methodargs omdef0))
+      ).
+      { rewrite map_Forall_lookup => x tx.
+        rewrite lookup_insert_Some.
+        case => [[? <-]|[?]] => //.
+        rewrite lookup_fmap_Some.
+        case => [tx' [ <- hx]].
+        apply wf_ty_subst.
+        - apply Forall_forall => tk hk.
+          apply elem_of_list_fmap_2 in hk as [tk2 [-> hk]].
+          apply wf_ty_subst => //.
+          rewrite Forall_forall in hwfot1.
+          by apply hwfot1 in hk.
+        - assert (ho0' := ho0).
+          apply wf_methods_wf in ho0'.
+          apply ho0' in hm0.
+          by apply hm0 in hx.
+      }
+      (* Use the induction hypothesis *)
+      iModIntro; iNext.
+      iSpecialize ("IH" $! _ _ _ wfbody hbody1 σi _ _ _ H11); simpl.
+      iDestruct ("IH" with "[Hh Hle H●]") as "Hstep".
+      { iSplit.
+        - iExists _; iFrame.
+          iSplit; first by rewrite Hdom.
+          done.
+        - iApply interp_local_tys_update => //; last first.
+            + rewrite interp_class_unfold /interp_class /=.
+              iExists l, t1, (gen_targs def1.(generics)), σt, fields, ifields; iSplitR.
+              { iPureIntro; repeat split => //; first by econstructor.
+                by rewrite subst_ty_gen_targs.
+              }
+              iSplit => //.
+              by iSplit.
+            + iApply interp_local_tys_list => //.
+              * destruct hincl0 as [hdomincl _].
+                rewrite !dom_fmap_L in hdomincl.
+                rewrite !dom_fmap_L in hdom.
+                by rewrite !dom_fmap_L hdomincl hdom.
+              * move => x ty arg.
+                rewrite lookup_fmap_Some.
+                case => [tx [<- hx]] harg.
+                destruct hincl1 as [hdom1 [hincl1 _]].
+                destruct (methodargs omdef !! x) as [ty' | ] eqn:hty'.
+                { assert (bounded (length σot) ty').
+                  { assert (ho' := ho).
+                    apply wf_methods_bounded in ho'.
+                    apply ho' in hom.
+                    apply hom in hty'.
+                    apply inherits_using_wf in hin => //.
+                    destruct hin as ( ? & ? & ? & ? & _ & hL & _); simplify_eq.
+                    by rewrite hL.
+                  }
+                  eapply ESubTy.
+                  - apply hi with x => //.
+                    by rewrite /subst_mdef /= lookup_fmap hty'.
+                  - apply wf_ty_subst.
+                    + rewrite Forall_forall => tk hk.
+                      apply elem_of_list_fmap_2 in hk as [tk2 [-> hk]].
+                      apply wf_ty_subst => //.
+                      rewrite Forall_forall in hwfot1; by apply hwfot1.
+                    + apply has_method_wf in hmorig0 as [hargs _] => //.
+                      by apply hargs in hx.
+                  - rewrite -!subst_ty_subst; first last.
+                    + apply bounded_subst with (length σot) => //.
+                      apply inherits_using_wf in hin => //.
+                      destruct hin as (? & ? & ? & ? & hF & _ & _).
+                      apply inherits_using_wf in hσin => //.
+                      destruct hσin as (? & ? & ? & ? & _ & hL' & _).
+                      simplify_eq.
+                      by rewrite hL'.
+                    + assert (ho0' := ho0).
+                      apply wf_methods_bounded in ho0'.
+                      apply ho0' in hm0.
+                      apply hm0 in hx.
+                      apply inherits_using_wf in hin1 => //.
+                      destruct hin1 as (? & ? & ? & ? & ? & hL' & _).
+                      simplify_eq.
+                      by rewrite hL'.
+                    + apply subtype_subst => //.
+                      rewrite subst_ty_subst //.
+                      apply hincl1 with x => //; first by rewrite /subst_mdef /= lookup_fmap hx.
+                      rewrite /subst_mdef /= fmap_subst_ty_subst //.
+                      by rewrite lookup_fmap hty'.
+                }
+                rewrite /subst_mdef /= !dom_fmap_L in hdom1.
+                apply mk_is_Some in hx.
+                apply elem_of_dom in hx.
+                rewrite hdom1 in hx.
+                apply elem_of_dom in hx.
+                rewrite hty' in hx.
+                by elim hx.
+      }
+      iRevert "Hstep".
       iApply updN_mono_I.
-      iIntros "[Hh Hle2]"; iFrame.
+      iIntros "[Hmodels Hle2]"; iFrame.
       iApply interp_local_tys_update; first by done.
-      destruct hincl as [? [? hret'']].
-      eapply subtype_subst in hret''.
-      iApply subtype_is_inclusion; first by apply hret''.
-      by iDestruct (expr_adequacy _ (methodret mdef0) with "Hle2") as "#Hret".
-         *)
+      destruct hincl1 as [? [? hret]].
+      iApply subtype_is_inclusion.
+      + done.
+      + done.
+      + done.
+      + rewrite -subst_ty_subst; last first.
+        * apply inherits_using_wf in hin => //.
+          destruct hin as ( ? & ? & ? & ? & hF & hL & _).
+          apply inherits_using_wf in hσin => //.
+          destruct hσin as (? & ? & ? & ? & hF' & hL' & _).
+          simplify_eq.
+          apply bounded_subst with odef.(generics) => //; last by rewrite hL'.
+          assert (ho' := ho).
+          apply wf_methods_bounded in ho'.
+          apply ho' in hom.
+          by apply hom.
+        * apply subtype_subst; first done; last done.
+          by apply hret.
+      + iDestruct (expr_adequacy _ (methodret omdef0) with "Hle2") as "#Hret" => //.
+        iClear "hifields_d hifields_s".
+        by rewrite subst_ty_subst.
     - (* Subtyping *) 
-      iIntros "H". iSpecialize ("IHty" with "[//] H").
+      destruct wfΔ.
+      iIntros "H".
+      iSpecialize ("IHty" $! wflty with "[//] H").
       iApply updN_mono_I; last done.
       iIntros "[Hh #Hrty]". iFrame.
       iDestruct (interp_local_tys_is_inclusion with "Hrty") as "Hrty'" => //.
-      { by apply wfΔ. }
       rewrite Forall_forall => i hi v.
       by apply _.
     - (* CondTagC *) inv hc; last first.
-      { by iApply updN_intro. }
+      { iIntros "[Hh H]".
+        iAssert (heap_models st'.2 ∗ interp_local_tys σi rty st'.1)%I with "[Hh H]" as "H".
+        + iFrame.
+          destruct wfΔ.
+          iApply interp_local_tys_is_inclusion => //.
+          rewrite Forall_forall => ???.
+          by apply _.
+        + iRevert "H".
+          by iApply updN_intro.
+      }
       iIntros "H".
-      iApply ("IHty" with "[//]"); iClear "IH IHty".
+      assert (hwf: map_Forall (λ _ : string, wf_ty) (<[v:=InterT tv (ExT t)]> lty)).
+      { rewrite map_Forall_lookup => k tk.
+        rewrite lookup_insert_Some.
+        case => [[? <-]|[? hk]].
+        + constructor; first by apply wflty in hv.
+          constructor.
+        + by apply wflty in hk.
+      }
+      iApply ("IHty" $! hwf with "[//]"); iClear "IH IHty".
       clear H6 h.
       destruct H5 as (l & hl & t' & fields & hlt & hinherits).
       iDestruct "H" as "[H #Hle]".
       iDestruct ("Hle" $! v with "[//]") as (?) "[%Hlev Hv]".
       rewrite Hlev in hl; simplify_eq.
-
       iAssert (interp_type MixedT σi (LocV l)) as "Hmixed".
-      { iApply subtype_is_inclusion; last done.
-        + by apply wfΔ.
-        + by apply SubMixed.
+      { destruct wfΔ.
+        iApply subtype_is_inclusion; [ done | done | done | by apply SubMixed | ].
+        done.
       }
       rewrite interp_mixed_unfold /=.
       iDestruct "Hmixed" as "[Hnonnull | Hnull]"; last first.
@@ -696,9 +724,9 @@ Section proofs.
       { iDestruct "Hint" as "%Hint"; by destruct Hint. }
       iDestruct "Hl" as "[Hbool | Hl]".
       { iDestruct "Hbool" as "%Hbool"; by destruct Hbool. }
-      iDestruct "Hl" as (exTag exσ k rt exfields ifields) "[%H [#Hfields #Hl]]".
-      destruct H as [[= <-] [hinherits' hfields']].
-      iAssert (heap_models st.2 ∗ interp_type (ExT exTag) σi (LocV l))%I with "[H]" as "[Hh #Hv2]".
+      iDestruct "Hl" as (exTag exσ k rt σ σt exfields ifields) "[%H [#Hfields_d [#hfields_s #Hl]]]".
+      destruct H as [[= <-] [hinherits' [hwf' [ heq' hfields']]]].
+      iAssert (⌜t' = rt⌝ ∗ heap_models st.2 ∗ interp_type (ExT rt) σi (LocV l))%I with "[H]" as "[%heq [Hh #Hv2]]".
       { iDestruct "H" as (sh) "(H● & %hdom & #Hh)".
         iDestruct (sem_heap_own_valid_2 with "H● Hl") as "#HΦ".
         iDestruct ("Hh" with "[//]") as (iFs) "[H H▷]".
@@ -706,13 +734,25 @@ Section proofs.
         rewrite option_equivI prod_equivI /=.
         iDestruct "HΦ" as "[%Ht HΦ]".
         fold_leibniz; subst.
+        iSplitR; first by iPureIntro.
         iSplitL. { iExists _. iFrame. by iSplit. }
         rewrite interp_ex_unfold /=.
-        iExists exσ, l, rt, exfields, ifields.
-        iSplit; first done.
-        by iSplit.
+        assert (hrt: is_Some(Δ !! rt)).
+        { inv hwf'.
+          by rewrite H1.
+        }
+        destruct hrt as [def hrt].
+        iExists σt, l, rt, (gen_targs def.(generics)), σt, exfields, ifields.
+        iSplit.
+        + iPureIntro; repeat split => //.
+          * by constructor.
+          * rewrite subst_ty_gen_targs //.
+            inv hwf'.
+            by simplify_eq.
+        + iSplit => //.
+          by iSplit.
       }
-      replace t' with rt in *; last by admit.
+      subst.
       iFrame.
       iIntros (w tw).
       rewrite lookup_insert_Some.
@@ -720,22 +760,22 @@ Section proofs.
       destruct Hw as [[<- <-] | [hne hw]].
       { iExists (LocV l); rewrite Hlev; iSplitR; first done.
         rewrite interp_inter_unfold /=; iSplit; first done.
-        by iApply inherits_is_inclusion.
+        destruct wfΔ.
+        by iApply inherits_is_ex_inclusion.
       }
       by iApply "Hle".
   Qed.
 
   Lemma cmd_adequacy (env: interp_env) lty cmd lty' :
     wf_cdefs Δ →
+    map_Forall (λ _ : string, wf_ty) lty →
     cmd_has_ty lty cmd lty' →
     ∀ st st' n, cmd_eval st cmd st' n →
     heap_models st.2 ∗ interp_local_tys env lty st.1 -∗ |=▷^n
         heap_models st'.2 ∗ interp_local_tys env lty' st'.1.
   Proof.
-    move => ? hty ??? hc.
-    iApply cmd_adequacy_; first done.
-    by iPureIntro.
-    by iPureIntro.
+    move => ?? hty ??? hc.
+    by iApply cmd_adequacy_.
   Qed.
 
 End proofs.
